theories/ast.v
@@ -1,6 +1,6 @@
-From Ssreflect
+From mathcomp
 Require Import ssreflect ssrfun ssrbool ssrnat eqtype choice seq fintype.
-From MathComp
+From mathcomp
 Require Import finfun finset generic_quotient.
 
 Require Import finmap finsfun finperm nominal utilitaires.
@@ -18,11 +18,11 @@ Import Key.Exports.
 
 Context (cons_label : eqType)
         (bcons_label : eqType)
-        (annot_label : nominalType atom).
+        (annot_label : {nominalType atom}).
 
 Section ASTDef.
 
-Inductive rAST := 
+Inductive rAST :=
 |rVar of atom
 |rAnnot of annot_label
 |rCons of cons_label & seq rAST
@@ -41,17 +41,17 @@ Canonical rAST_choiceType := ChoiceType rAST rAST_choiceMixin.
 Definition rAST_countMixin := CanCountMixin rAST_codeK.
 Canonical rAST_countType := CountType rAST rAST_countMixin.
 
-Lemma rAST_better_ind_subproof (P : rAST -> Prop) (f : seq rAST): 
+Lemma rAST_better_ind_subproof (P : rAST -> Prop) (f : seq rAST):
  foldr (fun t => and (P t)) True f -> (forall t, t \in f -> P t).
 Proof.
-elim: f => [|t l IHl] //=. 
-move => [Ptt P_all_l] u. 
+elim: f => [|t l IHl] //=.
+move => [Ptt P_all_l] u.
 rewrite inE => /orP. case; first by move /eqP ->.
 by apply IHl.
 Qed.
 
 Definition rAST_better_ind P IH_var IH_annot IH_cons IH_bcons :=
-  fix loop t : P t : Prop := 
+  fix loop t : P t : Prop :=
   let fix iter_conj f : foldr (fun t => and (P t)) True f :=
       if f is t :: f' then conj (loop t) (iter_conj f') else Logic.I
   in
@@ -78,8 +78,8 @@ Fixpoint rAST_act (π : {finperm atom}) (t : rAST) :=
     |rBinderCons c x l => rBinderCons c (π x) [seq (rAST_act π u) | u <- l]
   end.
 
-Lemma rAST_act1 : rAST_act (1 atom) =1 id.
-Proof. 
+Lemma rAST_act1 : rAST_act 1 =1 id.
+Proof.
 elim/rAST_better_ind => [x|a|c l IHl|c x l IHl] /=.
   - by rewrite finsfun1.
   - by rewrite act1.
@@ -87,15 +87,15 @@ elim/rAST_better_ind => [x|a|c l IHl|c x l IHl] /=.
   - by rewrite finsfun1 map_id_in.
 Qed.
 
-Lemma rAST_actM π π' (t : rAST) : 
+Lemma rAST_actM π π' (t : rAST) :
   rAST_act (π * π') t = rAST_act π (rAST_act π' t).
 Proof.
 elim/rAST_better_ind :t => [x|a|c l IHl|c x l IHl] /=.
   - by rewrite finsfunM.
   - by rewrite actM.
-  - congr rCons. rewrite -map_comp. 
+  - congr rCons. rewrite -map_comp.
     apply eq_in_map => t /=. exact: IHl.
-  - congr rBinderCons. 
+  - congr rBinderCons.
       by rewrite finsfunM.
     rewrite -map_comp. apply eq_in_map => t /=.
     exact: IHl.
@@ -104,9 +104,9 @@ Qed.
 Lemma rAST_actproper : forall t1 t2 π, t1 = t2 -> (rAST_act π t1) = (rAST_act π t2).
 Proof. by move => t1 t2 π ->. Qed.
 
-Definition rAST_nominal_setoid_mixin := 
-  @PermSetoidMixin rAST (@eq rAST) atom rAST_act rAST_act1 
-                   rAST_actM rAST_actproper.   
+Definition rAST_nominal_setoid_mixin :=
+  @PermSetoidMixin _ rAST (@eq rAST) rAST_act rAST_act1
+                   rAST_actM rAST_actproper.
 
 Fixpoint rAST_support t :=
   match t with
@@ -119,7 +119,7 @@ Fixpoint rAST_support t :=
 Lemma rAST_cons_support (l : seq rAST) (t : rAST) c :
   t \in l -> rAST_support t `<=` rAST_support (rCons c l).
 Proof.
-move => t_l. 
+move => t_l.
 apply/fsubsetP => x x_supp_t.
 apply/fsetU_listP. exists (rAST_support t) => //.
 exact: map_f.
@@ -128,7 +128,7 @@ Qed.
 Lemma rAST_bcons_support (l : seq rAST) (t : rAST) c y :
   t \in l -> rAST_support t `<=` rAST_support (rBinderCons c y l).
 Proof.
-move => t_l. 
+move => t_l.
 apply/fsubsetP => x x_supp_t /=.
 apply/fset1Ur/fsetU_listP. exists (rAST_support t) => //.
 exact: map_f.
@@ -138,51 +138,51 @@ Lemma rAST_act_id (π : {finperm atom}) (t : rAST) :
      (forall a : atom, a \in rAST_support t -> π a = a) -> rAST_act π t = t.
 Proof.
 elim/rAST_better_ind : t => [x|a|c l IHl|c x l IHl] Hsupp /=.
-  - by rewrite -atomactE act_id.                        
+  - by rewrite -atomactE act_id.
   - by rewrite act_id.
   - rewrite map_id_in // => t t_in_l.
     apply IHl => // a a_supp_t.
-    exact/Hsupp/(fsubsetP (rAST_cons_support c t_in_l) a). 
+    exact/Hsupp/(fsubsetP (rAST_cons_support c t_in_l) a).
   - rewrite map_id_in.
-      by rewrite Hsupp // fset1U1. 
+      by rewrite Hsupp // fset1U1.
     move => t t_in_l.
     apply IHl => // a a_supp_t.
-    exact/Hsupp/(fsubsetP (rAST_bcons_support c x t_in_l) a).     
+    exact/Hsupp/(fsubsetP (rAST_bcons_support c x t_in_l) a).
 Qed.
 
 End ASTDef.
 
 Definition rAST_nominal_mixin  :=
-  @NominalMixin rAST_choiceType  atom rAST_nominal_setoid_mixin _ 
+  @NominalMixin _ rAST rAST_nominal_setoid_mixin _
                 rAST_act_id.
 
-Canonical rAST_nominalType := 
-  @NominalType atom rAST_choiceType rAST_nominal_mixin.
+Canonical rAST_nominalType :=
+  NominalType atom rAST rAST_nominal_mixin.
 
 Section rDepth.
-  
-Lemma rdepth_cons_leq {c} {l} {n} : 
-  rAST_depth (rCons c l) <= n.+1 -> 
+
+Lemma rdepth_cons_leq {c} {l} {n} :
+  rAST_depth (rCons c l) <= n.+1 ->
   all (fun t : rAST  => rAST_depth t <= n) l.
 Proof.
 rewrite ltnS => /maxlist_leqP Hl.
-apply/allP => x xl. 
+apply/allP => x xl.
 exact/Hl/map_f.
 Qed.
 
-Lemma rdepth_bcons_leq {c} {l} {n} x : 
-  rAST_depth (rBinderCons c x l) <= n.+1 -> 
+Lemma rdepth_bcons_leq {c} {l} {n} x :
+  rAST_depth (rBinderCons c x l) <= n.+1 ->
   all (fun t : rAST  => rAST_depth t <= n) l.
 Proof.
 rewrite ltnS => /maxlist_leqP Hl.
-apply/allP => t tl. 
+apply/allP => t tl.
 exact/Hl/map_f.
 Qed.
 
-Lemma rdepth_perm (π : {finperm atom}) (t : rAST) : 
+Lemma rdepth_perm (π : {finperm atom}) (t : rAST) :
 rAST_depth (π \dot t) = rAST_depth t.
-Proof. 
-elim/rAST_better_ind: t => [x|a|? l ihl|? ? l ihl] //=. 
+Proof.
+elim/rAST_better_ind: t => [x|a|? l ihl|? ? l ihl] //=.
 all: apply eq_S; congr maxlist; rewrite -map_comp.
 all: apply eq_in_map => t tl /=.
 all: exact: ihl.
@@ -196,11 +196,11 @@ Fixpoint alpha_rec (n : nat) (W1 W2 : rAST ) :=
   match n, W1, W2 with
     |_, rVar x, rVar y => x == y
     |_, rAnnot a, rAnnot b => a == b
-    |S n, rCons c1 children1, rCons c2 children2 => 
-     (c1 == c2) && 
+    |S n, rCons c1 children1, rCons c2 children2 =>
+     (c1 == c2) &&
      (all2 (alpha_rec n) children1 children2)
     |S n, rBinderCons c1 x children1, rBinderCons c2 y children2 =>
-     (c1 == c2) && 
+     (c1 == c2) &&
      (let z := fresh_in (x, children1, y, children2) in
       all2 (alpha_rec n)
            (swap x z \dot children1)
@@ -208,27 +208,27 @@ Fixpoint alpha_rec (n : nat) (W1 W2 : rAST ) :=
     |_, _,_ => false
   end.
 
-Definition alpha W1 W2 := alpha_rec (rAST_depth W1) W1 W2.     
+Definition alpha W1 W2 := alpha_rec (rAST_depth W1) W1 W2.
 
-Lemma alpha_recE n (W1 W2 : rAST) : 
-  (rAST_depth W1 <= n) -> 
+Lemma alpha_recE n (W1 W2 : rAST) :
+  (rAST_depth W1 <= n) ->
   alpha_rec n W1 W2 = alpha W1 W2.
 Proof.
-rewrite /alpha; move: {-2}n (leqnn n). 
+rewrite /alpha; move: {-2}n (leqnn n).
 elim: n W1 W2 => // [|n ihn] [x|a|c1 l1|c1 x1 l1] [y|b|c2 l2|c2 x2 l2] [|m] //.
   - rewrite ltnS => m_leq_n /rdepth_cons_leq /allP IHl1 /=.
-    apply andb_id2l => _. 
+    apply andb_id2l => _.
     apply eq_in_all2 => t1 t2 t1l2 t2l2.
     rewrite !ihn //; last exact: IHl1.
-      apply/(@leq_trans m) => //. 
+      apply/(@leq_trans m) => //.
       exact/maxlist_map_leqP.
     exact/in_maxlist/map_f.
-  - rewrite ltnS => m_leq_n /rdepth_bcons_leq /allP IHl1 /=. 
-    apply andb_id2l => _. 
+  - rewrite ltnS => m_leq_n /rdepth_bcons_leq /allP IHl1 /=.
+    apply andb_id2l => _.
     apply eq_in_all2 => t1 t2 /mapP [?] ? -> /mapP [?] ? ->.
     rewrite !ihn //; try rewrite rdepth_perm; last exact/IHl1;
       last exact/in_maxlist/map_f.
-    apply (@leq_trans m) => //. 
+    apply (@leq_trans m) => //.
     exact/maxlist_map_leqP/IHl1.
 Qed.
 
@@ -240,28 +240,28 @@ Lemma alpha_VarE (x y : atom) :
   alpha (rVar x) (rVar y) = (x == y).
 Proof. by rewrite /alpha. Qed.
 
-Lemma alpha_AnnotE (a b : annot_label) : 
+Lemma alpha_AnnotE (a b : annot_label) :
   alpha (rAnnot a) (rAnnot b) = (a == b).
 Proof. by rewrite /alpha. Qed.
 
-Lemma alpha_ConsE (c1 c2 : cons_label) l1 l2 : 
+Lemma alpha_ConsE (c1 c2 : cons_label) l1 l2 :
   alpha (rCons c1 l1) (rCons c2 l2) = (c1 == c2) && all2 alpha l1 l2.
-Proof. 
-rewrite/alpha /=. 
+Proof.
+rewrite/alpha /=.
 apply andb_id2l => _. apply eq_in_all2 => t1 t2 ? ?.
-rewrite alpha_recE //. 
+rewrite alpha_recE //.
 exact/in_maxlist/map_f.
 Qed.
 
-Lemma alpha_BinderConsE (c1 c2 : bcons_label) x1 x2 l1 l2  : 
-  alpha (rBinderCons c1 x1 l1) (rBinderCons c2 x2 l2) = 
+Lemma alpha_BinderConsE (c1 c2 : bcons_label) x1 x2 l1 l2  :
+  alpha (rBinderCons c1 x1 l1) (rBinderCons c2 x2 l2) =
   (c1 == c2) &&
   let z := fresh_in (x1,l1,x2,l2) in
   all2 alpha (swap x1 z \dot l1) (swap x2 z \dot l2).
-Proof. 
-rewrite /alpha /=. 
-apply andb_id2l => _. 
-apply eq_in_all2 => t1 t2 /mapP [?] ? -> /mapP [?] ? ->. 
+Proof.
+rewrite /alpha /=.
+apply andb_id2l => _.
+apply eq_in_all2 => t1 t2 /mapP [?] ? -> /mapP [?] ? ->.
 rewrite alpha_recE // rdepth_perm.
 exact/in_maxlist/map_f.
 Qed.
@@ -274,9 +274,9 @@ Proof.
 rewrite/alpha rdepth_perm.
 move: {-1}(rAST_depth W1) (leqnn (rAST_depth W1)) => n.
 elim: n W1 W2 π => [|n IHn] [x1|a1|c1 l1|c1 x1 l1] [x2|a2|c2 l2|c2 x2 l2] π //=;
-  try solve [rewrite inj_eq //; exact: act_inj].
+  do ?by rewrite inj_eq //; do [apply/finperm_inj|apply/act_inj].
 all: rewrite ltnS => /maxlist_map_leqP IHl1.
-all: apply andb_id2l => _. 
+all: apply andb_id2l => _.
 all: rewrite !all2_map; apply eq_in_all2 => t1 t2 ? ?.
   exact/IHn/IHl1.
 set z := fresh_in _; set y := fresh_in _.
@@ -288,8 +288,8 @@ rewrite -{1}[t1](@act_fresh _ y (π^-1 z)) //; try freshTacList;
   last exact: im_inv_fresh.
 rewrite -{1}[t2](@act_fresh _ y (π^-1 z)) //; try freshTacList;
   last exact: im_inv_fresh. (* comment réécrire dans t1 et t2 à la fois ? *)
-rewrite 2?[in RHS]act_conj tfinpermL !tfinperm_fresh //.
-all: exact/im_inv_fresh. 
+do ?rewrite [swap y _ \dot _  \dot _]act_conj tfinpermL tfinperm_fresh //;
+   do?exact/im_inv_fresh.
 Qed.
 
 (* Lemma alpha_equivariantR {W1 W2 : rAST} {π1 π2 : {finperm atom}} x y : *)
@@ -302,7 +302,7 @@ Qed.
 Lemma alpha_equivariantprop : equivariant_prop alpha.
 Proof. move => π t t' /=. by rewrite alpha_equivariant. Qed.
 
-Lemma alpha_BConsP x1 x2 c1 c2 (l1 l2 : seq rAST) : 
+Lemma alpha_BConsP x1 x2 c1 c2 (l1 l2 : seq rAST) :
   reflect (c1 = c2 /\
            \new z, (all2 (fun t1 t2 => alpha (swap x1 z \dot t1)
                                             (swap x2 z \dot t2))
@@ -315,7 +315,7 @@ apply/(equivP andP); apply and_iff_congr => /=.
   by symmetry; apply (rwP eqP).
 rewrite all2_map.
 eapply iff_stepl. by symmetry; apply new_all2.
-eapply iff_stepl. by apply (rwP (@all2P _ _ _ _)). 
+eapply iff_stepl. by apply (rwP (@all2P _ _ _ _)).
 apply/eq_in_all2_prop => t1 t2 t1l1 t2l2.
 apply (@some_fresh_new _ _ Requi _ ((x1, t1), (x2, t2))).
 freshTac => *.
@@ -328,7 +328,7 @@ Proof.
 elim/rAST_better_ind => [x|a|c l|c x l]; rewrite alphaE eqxx //= => Hrefl.
 all: apply all2_refl => t.
   exact/Hrefl.
-move/mapP => [?] ? ->. 
+move/mapP => [?] ? ->.
 rewrite alpha_equivariant. exact/Hrefl.
 Qed.
 
@@ -345,21 +345,21 @@ all: apply all2_sym => t1 t2 t1l1 t2l2.
 all: rewrite /switch IHn ?rdepth_perm; last by apply depth_l1_leqn.
   exact/sym_eq/alpha_recE/in_maxlist/map_f.
 rewrite !alpha_recE; last first.
-  by rewrite rdepth_perm. 
+  by rewrite rdepth_perm.
   rewrite rdepth_perm; exact/in_maxlist/map_f.
 suff : fresh_in (x1, l1, x2, l2) = fresh_in (x2, l2, x1, l1) by move ->.
-suff : support (x1, l1, x2, l2) = support (x2, l2, x1, l1) 
-  by rewrite/fresh_in => ->. 
+suff : support (x1, l1, x2, l2) = support (x2, l2, x1, l1)
+  by rewrite/fresh_in => ->.
 repeat (rewrite/support/=).
-by rewrite -fsetUA fsetUC fsetUA. 
+by rewrite -fsetUA fsetUC fsetUA.
 Qed.
 
 Lemma alpha_trans : transitive alpha.
 move => t2 t1 t3.
 move: {-1}(rAST_depth t1) (leqnn (rAST_depth t1)) => n.
-elim: n t1 t2 t3 => [|n IHn] [x1|a1|c1 l1|c1 x1 l1] 
-                             [x2|a2|c2 l2|c2 x2 l2] 
-                             [x3|a3|c3 l3|c3 x3 l3] //=; 
+elim: n t1 t2 t3 => [|n IHn] [x1|a1|c1 l1|c1 x1 l1]
+                             [x2|a2|c2 l2|c2 x2 l2]
+                             [x3|a3|c3 l3|c3 x3 l3] //=;
 try solve [move => _; apply eq_op_trans].
 all: rewrite ltnS => /maxlist_map_leqP deptht1_leqn.
   rewrite !alphaE => /andP [c1_eq_c2 Hl1l2] /andP [c2_eq_c3 Hl2l3].
@@ -381,8 +381,8 @@ End AlphaEquivalence.
 
 Section Quotient.
 
-Canonical alpha_equiv := 
-  EquivRel alpha alpha_refl alpha_sym alpha_trans. 
+Canonical alpha_equiv :=
+  EquivRel alpha alpha_refl alpha_sym alpha_trans.
 
 Definition AST := {eq_quot alpha}.
 Definition AST_eqMixin := [eqMixin of AST].
@@ -390,19 +390,19 @@ Canonical AST_eqType := EqType AST AST_eqMixin.
 Canonical AST_choiceType := Eval hnf in [choiceType of AST].
 Canonical AST_countType := Eval hnf in [countType of AST].
 Canonical AST_quotType := Eval hnf in [quotType of AST].
-Canonical AST_eqQuotType := Eval hnf in 
+Canonical AST_eqQuotType := Eval hnf in
       [eqQuotType alpha of AST].
 
 Lemma alpha_eqE t t' : alpha t t' = (t == t' %[mod AST]).
 Proof. by rewrite piE. Qed.
 
-Lemma all2_alpha_eq l1 l2 : 
-  all2 alpha l1 l2 -> 
-  map \pi_AST l1 = map \pi_AST l2. 
+Lemma all2_alpha_eq l1 l2 :
+  all2 alpha l1 l2 ->
+  map \pi_AST l1 = map \pi_AST l2.
 Proof.
 move => /all2P alpha_l1l2. apply/all2_prop_eq/all2_prop_map.
 move : alpha_l1l2; apply eq_in_all2_prop => t1 t2 t1s1 t2s2.
-rewrite alpha_eqE. 
+rewrite alpha_eqE.
 by split; move/eqP.
 Qed.
 
@@ -414,13 +414,13 @@ Definition Annot a := lift_cst AST (rAnnot a).
 Lemma rAnnotK a : \pi_AST (rAnnot a) = Annot a.
 Proof. by unlock Annot. Qed.
 
-Notation lift_map f := 
+Notation lift_map f :=
   (locked (fun l : seq AST => \pi_AST (f (map (@repr _ AST_quotType) l)))).
 
 Definition Cons c := lift_map (rCons c).
 Lemma rConsK c l : \pi_AST (rCons c l) = Cons c (map \pi_AST l).
 Proof.
-unlock Cons; apply/eqP. 
+unlock Cons; apply/eqP.
 rewrite [_ == _]piE alphaE eqxx /= -map_comp.
 rewrite all2_mapr. apply all2_refl => t _ /=.
 by rewrite alpha_eqE reprK.
@@ -430,8 +430,8 @@ Definition BinderCons c x := lift_map (rBinderCons c x).
 Lemma rBinderConsK c x l : \pi_AST (rBinderCons c x l) = BinderCons c x (map \pi_AST l).
 Proof.
 unlock BinderCons; apply/eqP.
-rewrite [_ == _]piE alphaE eqxx /=. 
-rewrite all2_equivariant; 
+rewrite [_ == _]piE alphaE eqxx /=.
+rewrite all2_equivariant;
   last by move => ? ? ?; rewrite alpha_equivariant.
 rewrite -map_comp all2_mapr. apply all2_refl => t _ /=.
 by rewrite alpha_eqE reprK.
@@ -445,51 +445,51 @@ Implicit Types (π : {finperm atom}).
 
 Definition AST_act π (t : AST) := \pi_AST (π \dot repr t).
 
-Lemma AST_act1 : AST_act (1 atom) =1 id.
+Lemma AST_act1 : AST_act 1 =1 id.
 Proof. move => t /=. by rewrite /AST_act act1 reprK. Qed.
 
-Lemma AST_act_equiv π t : 
-  π \dot (repr t) == repr (AST_act π t) %[mod AST].   
+Lemma AST_act_equiv π t :
+  π \dot (repr t) == repr (AST_act π t) %[mod AST].
 Proof. by rewrite /AST_act reprK. Qed.
 
 Lemma AST_actM π π' t : AST_act (π * π') t = AST_act π (AST_act π' t).
 Proof.
-apply/eqP. 
-by rewrite /AST_act actM piE alpha_equivariant alpha_eqE reprK. 
+apply/eqP.
+by rewrite /AST_act actM piE alpha_equivariant alpha_eqE reprK.
 Qed.
 
-Lemma AST_actproper : 
+Lemma AST_actproper :
   forall t1 t2 π, t1 = t2 -> (AST_act π t1) = (AST_act π t2).
 Proof. by move => t1 t2 π ->. Qed.
 
 Definition AST_nominal_setoid_mixin :=
-  @PermSetoidMixin AST (@eq AST) atom AST_act AST_act1 AST_actM AST_actproper.
+  @PermSetoidMixin _ AST (@eq AST) AST_act AST_act1 AST_actM AST_actproper.
 
 Lemma AST_act_id π t :
-     (forall a : atom, a \in rAST_support (repr t) -> π a = a) -> 
+     (forall a : atom, a \in rAST_support (repr t) -> π a = a) ->
      AST_act π t = t.
 Proof.
 rewrite/AST_act => Hact_id.
-by rewrite act_id // reprK. 
+by rewrite act_id // reprK.
 Qed.
 
 Definition AST_nominal_mixin :=
-  @NominalMixin AST_choiceType atom AST_nominal_setoid_mixin _ AST_act_id.
+  @NominalMixin _ AST AST_nominal_setoid_mixin _ AST_act_id.
 
-Canonical AST_nominalType := @NominalType atom AST_choiceType AST_nominal_mixin.
+Canonical AST_nominalType := NominalType atom AST AST_nominal_mixin.
 
 End NominalAST.
 
 Section VariousLemmas.
 
-Lemma pi_equivariant π (t : rAST) : 
+Lemma pi_equivariant π (t : rAST) :
   π \dot (\pi_AST t) = \pi_AST (π \dot t).
 Proof.
-apply/eqmodP => /=. 
-by rewrite alpha_equivariant alpha_eqE reprK. 
+apply/eqmodP => /=.
+by rewrite alpha_equivariant alpha_eqE reprK.
 Qed.
 
-Lemma repr_equivariant π (t : AST) : repr (π \dot t) == π \dot (repr t) %[mod AST]. 
+Lemma repr_equivariant π (t : AST) : repr (π \dot t) == π \dot (repr t) %[mod AST].
 Proof. by rewrite -pi_equivariant !reprK. Qed.
 
 Lemma Var_equivariant π x : π \dot (Var x) = Var (π x).
@@ -498,10 +498,10 @@ Proof. by rewrite -rVarK pi_equivariant /= rVarK. Qed.
 Lemma Annot_equivariant π x : π \dot (Annot x) = Annot (π \dot x).
 Proof. by rewrite -rAnnotK pi_equivariant /= rAnnotK. Qed.
 
-Lemma Cons_equivariant π c l : 
+Lemma Cons_equivariant π c l :
   π \dot (Cons c l) = Cons c (π \dot l).
 Proof.
-unlock Cons. rewrite pi_equivariant !rConsK -!map_comp. 
+unlock Cons. rewrite pi_equivariant !rConsK -!map_comp.
 congr Cons.
 apply/sym_eq/eq_map => t /=.
 exact/eqP/repr_equivariant.
@@ -533,7 +533,7 @@ Qed.
 Lemma fresh_list_repr x (l : seq AST) : x # (map repr l) -> x # l.
 Proof.
 move => ?.
-apply fresh_list => ? /(map_f (@repr rAST AST_quotType)) ?. 
+apply fresh_list => ? /(map_f (@repr rAST AST_quotType)) ?.
 apply fresh_repr; by freshTacList.
 Qed.
 
@@ -545,12 +545,12 @@ Qed.
 
 Lemma eq_BConsE c x1 x2 l1 l2 :
   BinderCons c x1 l1 = BinderCons c x2 l2 ->
-  forall z, z # x1 -> z # x2 -> z # l1 -> z # l2 -> 
+  forall z, z # x1 -> z # x2 -> z # l1 -> z # l2 ->
              swap x2 z \dot l2 = swap x1 z \dot l1.
 Proof.
-unlock BinderCons => /eqP. 
+unlock BinderCons => /eqP.
 rewrite -alpha_eqE alphaE eqxx /= => /all2_alpha_eq.
-set z := fresh_in _. 
+set z := fresh_in _.
 rewrite -!map_equivariant;
   try solve [move => *; exact: pi_equivariant].
 rewrite !mapK;
@@ -558,34 +558,34 @@ rewrite !mapK;
 move => x1zl1_x2zl2 z' *.
 freshTacCtxt z.
 apply (@act_inj _ _ (swap z z')).
-rewrite [in LHS]act_conj [in RHS]act_conj !tfinpermR !tfinperm_fresh //. 
+rewrite [in LHS]act_conj [in RHS]act_conj !tfinpermR !tfinperm_fresh //.
 rewrite ![swap z z' \dot _]act_fresh //.
 all: exact: fresh_list_repr.
 Qed.
 
-Lemma VarK x : repr (Var x) = rVar x. 
+Lemma VarK x : repr (Var x) = rVar x.
 Proof.
-have : alpha (repr (Var x)) (rVar x). 
-  by rewrite alpha_eqE reprK rVarK. 
-by case: (repr (Var x)) => // ? /eqP ->. 
+have : alpha (repr (Var x)) (rVar x).
+  by rewrite alpha_eqE reprK rVarK.
+by case: (repr (Var x)) => // ? /eqP ->.
 Qed.
 
-Lemma AnnotK x : repr (Annot x) = rAnnot x. 
+Lemma AnnotK x : repr (Annot x) = rAnnot x.
 Proof.
-have : alpha (repr (Annot x)) (rAnnot x). 
-  by rewrite alpha_eqE reprK rAnnotK. 
-by case: (repr (Annot x)) => // ? /eqP ->. 
+have : alpha (repr (Annot x)) (rAnnot x).
+  by rewrite alpha_eqE reprK rAnnotK.
+by case: (repr (Annot x)) => // ? /eqP ->.
 Qed.
 
 Lemma ConsK c l : exists repr_l,
     l = map \pi_AST repr_l /\ repr (Cons c l) = rCons c repr_l.
 Proof.
 have: alpha (repr (Cons c l)) (rCons c (map repr l)).
-  rewrite alpha_eqE reprK rConsK -map_comp map_id_in //. 
+  rewrite alpha_eqE reprK rConsK -map_comp map_id_in //.
   move => t _ /=. by rewrite reprK.
 case: (repr (Cons _ _)) => //= c2 l2;
-rewrite alphaE // => /andP [/eqP c2_eq_c] => /all2_alpha_eq. 
-rewrite -map_comp map_id_in => pil2_ll1; 
+rewrite alphaE // => /andP [/eqP c2_eq_c] => /all2_alpha_eq.
+rewrite -map_comp map_id_in => pil2_ll1;
   last by move => _ /=; rewrite reprK.
 by exists l2; split; last by rewrite c2_eq_c.
 Qed.
@@ -594,11 +594,11 @@ Lemma BConsK c (x : atom) (l : seq AST) : exists (y : atom) (repr_l : seq rAST),
    repr (BinderCons c x l) = rBinderCons c y repr_l.
 Proof.
 have: alpha (repr (BinderCons c x l)) (rBinderCons c x (map repr l)).
-  rewrite alpha_eqE reprK rBinderConsK -map_comp map_id_in //. 
+  rewrite alpha_eqE reprK rBinderConsK -map_comp map_id_in //.
   move => t _ /=. by rewrite reprK.
 case: (repr (BinderCons _ _ _)) => //= c2 x2 l2.
-rewrite alphaE => /andP [/eqP ->] /= H. 
-by exists x2; exists l2. 
+rewrite alphaE => /andP [/eqP ->] /= H.
+by exists x2; exists l2.
 Qed.
 
 Lemma AST_caseP (t : AST) :
@@ -609,46 +609,46 @@ Lemma AST_caseP (t : AST) :
 Proof.
 case_eq (repr t) => [x|a|c l|c x l] /(congr1 \pi_AST).
 all: rewrite reprK (rVarK, rAnnotK, rConsK, rBinderConsK) => ?.
-  - left. by exists x.                                                            
+  - left. by exists x.
   - right; left. by exists a.
   - right; right; left. by exists c; exists (map \pi l).
   - right; right; right. by exists c; exists x; exists (map \pi l).
 Qed.
 
 Lemma Var_inj : injective Var.
-Proof. 
+Proof.
 move => x y /(congr1 repr). rewrite !VarK => H. by injection H. Qed.
 
 Lemma Annot_inj : injective Annot.
-Proof. 
+Proof.
 move => x y /(congr1 repr). rewrite !AnnotK => H. by injection H. Qed.
 
-Lemma Cons_inj c1 c2 l1 l2 : 
+Lemma Cons_inj c1 c2 l1 l2 :
   Cons c1 l1 = Cons c2 l2 -> c1 = c2 /\ l1 = l2.
 Proof.
-move/(congr1 repr). 
+move/(congr1 repr).
 have [reprl1 [-> ->]] := ConsK c1 l1.
 have [reprl2 [-> ->]] := ConsK c2 l2.
 move => H.
-by injection H => -> ->. 
+by injection H => -> ->.
 Qed.
 
 Lemma BConsx_inj c x : injective (BinderCons c x).
 Proof.
-move => l1 l2; 
-pose z := fresh_in (x, l1, l2). 
+move => l1 l2;
+pose z := fresh_in (x, l1, l2).
 move => /eq_BConsE /(_ (fresh_in (x, l1, l2))) H.
 apply/(@act_inj _ _ (swap x z))/sym_eq.
 freshTacCtxt z.
 exact/H.
-Qed. 
+Qed.
 
 Lemma fresh_Var x y : x # (Var y) <-> x # y.
 Proof.
 split => [[S] [xNS S_supp_Ly]|xFy].
   exists S; split => // π HS.
   apply Var_inj. rewrite -Var_equivariant.
-  exact: S_supp_Ly.   
+  exact: S_supp_Ly.
 apply (@CFN_principle (fresh_in (y, Var y))); first by freshTac.
 rewrite Var_equivariant tfinperm_fresh //; by freshTac.
 Qed.
@@ -658,7 +658,7 @@ Proof.
 split => [[S] [xNS S_supp_Ly]|xFy].
   exists S; split => // π HS.
   apply Annot_inj. rewrite -Annot_equivariant.
-  exact: S_supp_Ly.   
+  exact: S_supp_Ly.
 apply (@CFN_principle (fresh_in (y, Annot y))); first by freshTac.
 rewrite Annot_equivariant act_fresh //; by freshTac.
 Qed.
@@ -671,21 +671,21 @@ eapply proj2; apply Cons_inj. rewrite -Cons_equivariant.
 exact: S_supp_cl.
 Qed.
 
-Lemma fresh_rBCons x y c (l : seq rAST) : 
+Lemma fresh_rBCons x y c (l : seq rAST) :
   x # (rBinderCons c y l) -> x # y /\ x # l.
-Proof.                             
+Proof.
 move => [S] [xNS S_supp_cyl].
 split; exists S; split => // π Hπ.
 all: by move: (S_supp_cyl π Hπ) => /= H; injection H => *.
 Qed.
 
-Lemma fresh_BCons x y c l : 
+Lemma fresh_BCons x y c l :
   x # y -> x # (BinderCons c y l) -> x # l.
 Proof.
 move => [S] [xNS S_supp_y] [S'] [xNS' S'_supp_cyl].
 exists (S `|` S'); split.
   by rewrite in_fsetU negb_or xNS xNS'.
-move => π Hπ. 
+move => π Hπ.
 apply/(@BConsx_inj c y).
 have y_eq_piy : π y = y.
   apply S_supp_y => a aS. apply Hπ.
@@ -694,13 +694,13 @@ rewrite -{1}y_eq_piy -BinderCons_equivariant.
 apply S'_supp_cyl => a aS'. apply Hπ.
 by rewrite in_fsetU aS' orbT.
 Qed.
-  
+
 Lemma eq_BCons c x y l :
   y # x -> y # l -> BinderCons c x l = BinderCons c y (swap x y \dot l).
 Proof.
 move => xFy xFl.
 unlock BinderCons; apply/eqmodP => /=.
-rewrite alphaE eqxx /= !all2_map all2_mapr. 
+rewrite alphaE eqxx /= !all2_map all2_mapr.
 apply all2_refl => t tl; set z := fresh_in _; freshTacCtxt z.
 rewrite alpha_eqE -!pi_equivariant !reprK.
 rewrite act_conj tfinpermL tfinperm_fresh //.
@@ -709,7 +709,7 @@ move: tl => /(map_f (@repr rAST AST_quotType)) /= ?.
 apply fresh_repr; by freshTacList.
 Qed.
 
-Lemma bname_fresh x c l : x # (BinderCons c x l).
+Lemma bname_fresh (x : atom) c l : x # (BinderCons c x l).
 Proof.
 pose y := fresh_in (x, l, BinderCons c x l); freshTacCtxt y.
 apply (@CFN_principle y) => //.
@@ -723,22 +723,22 @@ Section Depth.
 
 Definition depth (t : AST) := rAST_depth (repr t).
 
-Lemma rdepth_alpha t u : alpha t u -> rAST_depth t = rAST_depth u. 
+Lemma rdepth_alpha t u : alpha t u -> rAST_depth t = rAST_depth u.
 Proof.
 elim/rAST_better_ind: t u => [x1|a1|c1 l1 IHl1|c1 x1 l1 IHl1] [x2|a2|c2 l2|c2 x2 l2] //=.
 all: rewrite alphaE => /andP /= [_ l1_alpha_l2].
 all: apply eq_S; congr maxlist.
-  apply (@all2_quot _ _ _ _ alpha) => // x y xl1 yl2. 
+  apply (@all2_quot _ _ _ _ alpha) => // x y xl1 yl2.
   exact/IHl1.
-eapply (@all2_quot _ _ _ _ ); last by 
+eapply (@all2_quot _ _ _ _ ); last by
   move: l1_alpha_l2; rewrite all2_map; exact: id.
 move => t1 t2 t1l1 t2l2 /=; set z:= fresh_in _.
 rewrite -(alpha_equivariant _ _ (swap x1 z)) -actM tfinperm_idempotent act1.
 by move/IHl1; rewrite !rdepth_perm; auto.
 Qed.
-                                                     
+
 Lemma depth_rdepth t : depth (\pi t) = rAST_depth t.
-Proof. 
+Proof.
 apply rdepth_alpha. by rewrite alpha_eqE reprK.
 Qed.
 
@@ -780,10 +780,10 @@ Lemma AST_naive_ind (P : AST -> Prop) :
   (forall c x l, (forall t, t \in l -> P t) -> P (BinderCons c x l)) ->
   forall u, P u.
 (* {in l, P} ? *)
-Proof. 
+Proof.
 move => HVar HAnnot HCons HBCons u; rewrite -[u]reprK.
 elim/rAST_better_ind : (repr u) => [x|a|c l IHl|c x l IHl] /=.
-  - by rewrite rVarK.              
+  - by rewrite rVarK.
   - by rewrite rAnnotK.
   - rewrite rConsK. apply HCons => t /mapP [reprt ?] ->.
     exact/IHl.
@@ -791,30 +791,30 @@ elim/rAST_better_ind : (repr u) => [x|a|c l IHl|c x l IHl] /=.
     exact/IHl.
 Qed.
 
-Lemma AST_ind {env : nominalType atom} (C : env) (P : AST -> Prop) :
+Lemma AST_ind {env : {nominalType atom}} (C : env) (P : AST -> Prop) :
   (forall x, P (Var x)) ->
   (forall x, P (Annot x)) ->
   (forall c l, (forall t, t \in l -> P t) -> P (Cons c l)) ->
   (forall c x l, x # C -> (forall t, t \in l -> P t) -> P (BinderCons c x l)) ->
   forall u, P u.
 (* {in l, P} ? *)
-Proof. 
+Proof.
 move => HVar HAnnot HCons HBcons u.
 suff : forall π, P (π \dot u).
-  by move => /(_ (1 atom)); rewrite act1.
+  by move => /(_ 1); rewrite act1.
 elim/AST_naive_ind : u => [x|a|c l IHl|c x l IHl] π.
   - by rewrite Var_equivariant.
   - by rewrite Annot_equivariant.
-  - rewrite Cons_equivariant. apply HCons => t /mapP [reprt ?] ->. 
-    exact/IHl.    
-  - rewrite BinderCons_equivariant. 
-    pose z := fresh_in (C, π x, π \dot l); freshTacCtxt z.
+  - rewrite Cons_equivariant. apply HCons => t /mapP [reprt ?] ->.
+    exact/IHl.
+  - rewrite BinderCons_equivariant.
+    pose z := fresh_in (C, π \dot x, π \dot l); freshTacCtxt z.
     rewrite (@eq_BCons _ _ z) -?actM => //.
     apply HBcons => // t /mapP [reprt ?] ->.
     exact/IHl.
 Qed.
 
-Variables (X : nominalType atom)
+Variables (X : {nominalType atom})
           (f_var : atom -> X)
           (f_annot : annot_label -> X)
           (f_cons : cons_label -> seq AST -> seq X -> X)
@@ -822,24 +822,24 @@ Variables (X : nominalType atom)
           (Supp : {fset atom})
           (dflt : X).
 
-Hypothesis f_var_equivariant : 
-  forall (π : {finperm atom}) x, 
+Hypothesis f_var_equivariant :
+  forall (π : {finperm atom}) x,
     [disjoint finsupp π & Supp] -> π \dot f_var x = f_var (π \dot x).
 
-Hypothesis f_annot_equivariant : 
-  forall (π : {finperm atom}) x, 
+Hypothesis f_annot_equivariant :
+  forall (π : {finperm atom}) x,
     [disjoint finsupp π & Supp] -> π \dot f_annot x = f_annot (π \dot x).
 
 Hypothesis f_cons_equivariant :
   forall (π : {finperm atom}) c l l',
     [disjoint finsupp π & Supp] ->
-                  π \dot f_cons c l l' = 
+                  π \dot f_cons c l l' =
                   f_cons c (π \dot l) (π \dot l').
 
 Hypothesis f_bcons_equivariant :
-  forall (π : {finperm atom}) c x l l', 
-    [disjoint finsupp π & Supp] -> π \dot f_bcons c x l l' = 
-                                   f_bcons c (π x) (π \dot l) (π \dot l').                 
+  forall (π : {finperm atom}) c x l l',
+    [disjoint finsupp π & Supp] -> π \dot f_bcons c x l l' =
+                                   f_bcons c (π x) (π \dot l) (π \dot l').
 
 Hypothesis FCB_fbcons :
   forall x c l l', x # Supp -> x # (f_bcons c x l l').
@@ -863,7 +863,7 @@ Definition AST_rect t := AST_rect_rec (depth t) t.
 Lemma AST_rect_recE n t : depth t <= n -> AST_rect_rec n t = AST_rect t.
 Proof.
 rewrite/AST_rect; move: {-2}n (leqnn n).
-elim: n t => [|n IHn] t //; rewrite /depth. 
+elim: n t => [|n IHn] t //; rewrite /depth.
   by move => ?; do 2?(rewrite leqn0 => /eqP ->).
 move => [?|m]; first by rewrite leqn0 => /eqP ->.
 rewrite ltnS => m_leq_n.
@@ -881,27 +881,27 @@ Proof. by rewrite /AST_rect depth_Var /= VarK. Qed.
 Lemma AST_rect_AnnotE x : AST_rect (Annot x) = f_annot x.
 Proof. by rewrite /AST_rect depth_Annot /= AnnotK. Qed.
 
-Lemma AST_rect_ConsE c l : 
+Lemma AST_rect_ConsE c l :
   AST_rect (Cons c l) = f_cons c l (map AST_rect l).
 Proof.
 rewrite/AST_rect depth_Cons /=.
 have [reprl [-> ->]] := ConsK c l.
 congr f_cons => //.
 rewrite -!map_comp. apply eq_in_map => t /= ?.
-apply AST_rect_recE => /=. 
+apply AST_rect_recE => /=.
 exact/in_maxlist/map_f.
 Qed.
 
 Lemma AST_rect_BConsE_subproof c x l :
   let z := (fresh_in (Supp, repr (BinderCons c x l))) in
-    AST_rect (BinderCons c x l) = 
+    AST_rect (BinderCons c x l) =
     f_bcons c z (swap x z \dot l) (map AST_rect (swap x z \dot l)).
 have [y [l'] repr_cxl] := BConsK c x l => /=.
 rewrite /AST_rect depth_BinderCons /= repr_cxl.
-set z := fresh_in _. 
+set z := fresh_in _.
 suff : swap y z \dot (map \pi_AST l') = swap x z \dot l.
   move => ->. congr f_bcons.
-  apply eq_in_map => ? /mapP [?] ? ->. 
+  apply eq_in_map => ? /mapP [?] ? ->.
   rewrite AST_rect_recE // depth_perm. exact/in_maxlist/map_f.
 move: (congr1 \pi_AST repr_cxl).
 rewrite reprK rBinderConsK => /eq_BConsE /(_ z) H.
@@ -910,36 +910,36 @@ move => /fresh_rBCons [? /fresh_list_pi ?].
 have [/eqP z_eq_x|/fresh_atomP ?] := boolP (z == x).
   rewrite z_eq_x tfinperm_id act1.
   move: (congr1 \pi_AST repr_cxl); rewrite reprK rBinderConsK.
-  rewrite [X in _ = X](@eq_BCons c y x) -?z_eq_x // => J.  
+  rewrite [X in _ = X](@eq_BCons c y x) -?z_eq_x // => J.
   exact/BConsx_inj/sym_eq/J.
 apply H => //. apply/(@fresh_BCons _ x c) => //.
-apply fresh_repr; rewrite repr_cxl. 
+apply fresh_repr; rewrite repr_cxl.
 by freshTac.
 Qed.
 
-Definition equiv t := 
+Definition equiv t :=
   forall (π : {finperm atom}), [disjoint finsupp π & Supp] ->
-                               π \dot (AST_rect t) = 
+                               π \dot (AST_rect t) =
                                AST_rect (π \dot t).
 
 Definition res c x l := AST_rect (BinderCons c x l) =
                         f_bcons c x l (map AST_rect l).
 
-Lemma equiv_res_subproof c x (l : seq AST) :
+Lemma equiv_res_subproof c (x : atom) (l : seq AST) :
 (forall (t : AST), t \in l -> equiv t) ->
 x # Supp -> res c x l.
 Proof.
 move => Hequiv zFSupp.
 rewrite /res AST_rect_BConsE_subproof; set y := fresh_in _.
 set rhs := RHS; set lhs := LHS; rewrite /lhs/rhs.
-set a := fresh_in (lhs, rhs, Supp, l, x). 
+set a := fresh_in (lhs, rhs, Supp, l, x).
 freshTacCtxt a. freshTacCtxt y.
 rewrite -[LHS](@act_fresh _ y a) //; last exact/FCB_fbcons.
 rewrite -[RHS](@act_fresh _ x a) //; last exact/FCB_fbcons.
 rewrite !f_bcons_equivariant;
-  try solve [exact/disjoint_tfsupp]. 
+  try solve [exact/disjoint_tfsupp].
 rewrite !tfinpermL.
-rewrite -map_equivariant; 
+rewrite -map_equivariant;
   last by move => ? ?; apply/Hequiv => //; apply/disjoint_tfsupp.
 have : y # BinderCons c x l by apply/fresh_repr.
 have [/eqP ->|/fresh_atomP zFx /(fresh_BCons zFx) ?] := boolP (y == x).
@@ -957,27 +957,26 @@ Proof.
 elim/(@AST_ind _ Supp): t => [v|a|c l IHl|c z l zFSupp IHl] π disj_pi_S.
   - by rewrite Var_equivariant !AST_rect_VarE f_var_equivariant.
   - by rewrite !Annot_equivariant !AST_rect_AnnotE f_annot_equivariant.
-  - rewrite !Cons_equivariant !AST_rect_ConsE f_cons_equivariant //. 
+  - rewrite !Cons_equivariant !AST_rect_ConsE f_cons_equivariant //.
     rewrite [X in f_cons _ _ X]map_equivariant //; last by
       move => t tl; exact/IHl.
   - have Hres1 := (@equiv_res_subproof c _ _ IHl zFSupp).
     have Hres2 : res c (π z) (π \dot l).
-      apply/equiv_res_subproof => //; last exact/disj_im_fresh. 
+      apply/equiv_res_subproof => //; last exact/disj_im_fresh.
       move => t /mapP [?] ? -> π' ?.
       rewrite -actM -!IHl // ?actM //; exact/disjoint_conj.
-    rewrite BinderCons_equivariant Hres1 Hres2. 
+    rewrite BinderCons_equivariant Hres1 Hres2.
     rewrite f_bcons_equivariant // map_equivariant // => ? ?.
     exact/IHl.
 Qed.
 
-Lemma AST_rect_BinderConsE c x l : 
-  x # Supp -> 
+Lemma AST_rect_BinderConsE c x l :
+  x # Supp ->
   AST_rect (BinderCons c x l) = f_bcons c x l (map AST_rect l).
 Proof.
 move => xFsupp.
-apply/equiv_res_subproof => // ? ?. 
+apply/equiv_res_subproof => // ? ?.
 exact/AST_rect_equivariant.
 Qed.
 
 End EliminationPrinciples.
-
