theories/finperm.v
@@ -1,7 +1,7 @@
-From Ssreflect
+From mathcomp
 Require Import ssreflect ssrfun ssrbool ssrnat eqtype choice seq fintype.
 
-From MathComp
+From mathcomp
 Require Import bigop  finfun finset generic_quotient perm tuple fingroup.
 Require Import finmap.
 Require Import finsfun.
@@ -33,16 +33,16 @@ Lemma finperm_inj (π : finPerm) : injective π.
 Proof. by case:π => *; apply/injectiveb_finsfunP. Qed.
 
 Lemma in_permsupp (π : finPerm) : {mono π : a / a \in finsupp π}.
-Proof. 
+Proof.
 move=> a; case: π => f /=.
 move=> /andP [/finsfun_injective_inP f_inj_in /forallP f_stable].
 by case: (finsuppP _ a) => [/negPf -> //|af]; apply: (f_stable (FSetSub af)).
 Qed.
 
 Lemma perm_stable (π : finPerm) (S : {fset K}) :
-  finsupp π `<=` S -> forall (a : K), a \in S -> π a \in S. 
+  finsupp π `<=` S -> forall (a : K), a \in S -> π a \in S.
 Proof.
-move=> /fsubsetP S_surfinsupp a; case:finsuppP; first by []. 
+move=> /fsubsetP S_surfinsupp a; case:finsuppP; first by [].
 by move => a_supp aS; apply/S_surfinsupp/(monoW (@in_permsupp _)).
 Qed.
 
@@ -53,7 +53,7 @@ Lemma eq1_finPermP (π π' : finPerm) : reflect (π =1 π') (eq_finPerm π π').
 Proof.
 apply: (iffP idP); last first.
   move => π_eq_π'. apply/forallP => *. by apply/eqP/π_eq_π'.
-move => /forallP π_eq_π' a. 
+move => /forallP π_eq_π' a.
 have [aππ'|aNππ'] := boolP (a \in (finsupp π `|` finsupp π')).
   by apply/eqP/(π_eq_π' (FSetSub aππ')).
 move:aNππ'; rewrite in_fsetU negb_or => /andP [aNπ aNπ'].
@@ -65,7 +65,7 @@ Proof.
 split; last by move ->.
 case: π; case: π' => f f_inj g g_inj g_eq1_f.
 suff g_eq_f : g = f.
-  move: g_eq_f f_inj g_inj g_eq1_f-> => f_inj g_inj _. congr FinPerm. 
+  move: g_eq_f f_inj g_inj g_eq1_f-> => f_inj g_inj _. congr FinPerm.
   exact: bool_irrelevance.
 by apply/finsfunP.
 Qed.
@@ -74,38 +74,38 @@ Lemma eq_finPerm_is_equiv : equiv_class_of eq_finPerm.
 Proof.
 split=> [p|p q|q p r].
   rewrite /eq_finPerm. by apply/forallP.
-  rewrite /eq_finPerm. apply/forallP/forallP => H; rewrite fsetUC => x; by rewrite eq_sym. 
+  rewrite /eq_finPerm. apply/forallP/forallP => H; rewrite fsetUC => x; by rewrite eq_sym.
 move=> /eq1_finPermP pq /eq1_finPermP qr.
 by apply/eq1_finPermP => n; rewrite pq qr.
 Qed.
 
 End FinPermDef.
 
-Notation "{finperm K }" := (@finperm_of _ (Phant K)) : type_scope.
+Notation "{finperm  K }" := (@finperm_of _ (Phant K)) : type_scope.
 
 Section PermFinPerm.
 
 Variable (K : keyType).
 
-Definition ffun_of_finPerm (π : {finperm K}) (S : {fset K}) 
-           (supp_incl_S : finsupp π `<=` S) := 
+Definition ffun_of_finPerm (π : {finperm K}) (S : {fset K})
+           (supp_incl_S : finsupp π `<=` S) :=
   [ffun x:S => FSetSub (perm_stable supp_incl_S (fsvalP x))].
 
-Fact perm_of_finPerm_subproof (π : {finperm K}) (S : {fset K}) 
-      (supp_incl_S : finsupp π `<=` S) : injectiveb (ffun_of_finPerm supp_incl_S). 
+Fact perm_of_finPerm_subproof (π : {finperm K}) (S : {fset K})
+      (supp_incl_S : finsupp π `<=` S) : injectiveb (ffun_of_finPerm supp_incl_S).
 Proof.
-apply/injectiveP => a b; rewrite !ffunE; move/(congr1 val) => πa_eq_πb. 
+apply/injectiveP => a b; rewrite !ffunE; move/(congr1 val) => πa_eq_πb.
 by apply/val_inj/(finperm_inj πa_eq_πb).
 Qed.
 
-Definition perm_of_finPerm (π : {finperm K}) (S : {fset K}) 
-           (supp_incl_S : finsupp π `<=` S) := 
+Definition perm_of_finPerm (π : {finperm K}) (S : {fset K})
+           (supp_incl_S : finsupp π `<=` S) :=
   Perm (perm_of_finPerm_subproof supp_incl_S).
 
-Definition can_perm_of_finPerm (π : {finperm K}) := 
+Definition can_perm_of_finPerm (π : {finperm K}) :=
   perm_of_finPerm (fsubsetAA (finsupp π)).
 
-Lemma perm_of_finPermE (π : {finperm K}) (S : {fset K}) 
+Lemma perm_of_finPermE (π : {finperm K}) (S : {fset K})
       (supp_incl_S : finsupp π `<=` S) :
   forall a : S, perm_of_finPerm supp_incl_S a = FSetSub (perm_stable supp_incl_S (fsvalP a)).
 Proof. move => a. by rewrite/perm_of_finPerm -pvalE /ffun_of_finPerm /= ffunE. Qed.
@@ -115,17 +115,17 @@ End PermFinPerm.
 Section FinPermSpec.
 
 Variable (K : keyType).
-  
+
 Lemma finPerm_can (π : {finperm K}) (a : K) (aπ : a \in finsupp π) :
   π a = (val (can_perm_of_finPerm π (FSetSub aπ))).
 Proof.
-have t : π a = val (FSetSub (perm_stable (fsubsetAA (finsupp π)) aπ)) by []. 
-by rewrite t perm_of_finPermE. 
+have t : π a = val (FSetSub (perm_stable (fsubsetAA (finsupp π)) aπ)) by [].
+by rewrite t perm_of_finPermE.
 Qed.
 
 CoInductive finPerm_spec (π : {finperm K}) (a : K) : K -> bool -> Type :=
   | FinPermOut : a \notin finsupp π -> finPerm_spec π a a false
-  | FinPermIn  (aπ : a \in finsupp π) : 
+  | FinPermIn  (aπ : a \in finsupp π) :
       finPerm_spec π a (val (can_perm_of_finPerm π (FSetSub aπ))) true.
 
 Lemma finPermP (π : {finperm K}) (a : K) : finPerm_spec π a (π a) (a \in finsupp π).
@@ -162,12 +162,12 @@ apply/andP. split; last first.
 apply/injectiveP => a b. rewrite !ffunE !finsfun_of_can_ffunE; rewrite ?ssvalP //=.
 move => bπ aπ. rewrite !ffunE => pa_eq_pb.
 suff: {| fsval := fsval a; fsvalP := aπ |} = {| fsval := fsval b; fsvalP := bπ |}.
-  by move/(congr1 val) => /=; apply/val_inj. 
+  by move/(congr1 val) => /=; apply/val_inj.
 apply/eqP. rewrite -(inj_eq (@perm_inj _ (perm_inv (can_perm_of_finPerm π)))).
 exact/eqP/val_inj.
 Qed.
 
-Definition finperm_inv := 
+Definition finperm_inv :=
   FinPerm injective_finsfun_subproof.
 
 Lemma finperm_one_subproof : injectiveb_finsfun_id (@finsfun_one K).
@@ -175,7 +175,7 @@ Proof. by apply/injectiveb_finsfunP/inj_finsfun_one. Qed.
 
 Definition finperm_one := FinPerm finperm_one_subproof.
 
-End FinPermInvDef. 
+End FinPermInvDef.
 
 Section FinPermMulDef.
 
@@ -190,29 +190,29 @@ Definition finperm_mul (π π' : {finperm K}) :=
 
 End FinPermMulDef.
 
-Notation "1" := (finperm_one).
+Notation "1" := (@finperm_one _).
 Notation "π * π'" := (@finperm_mul _ π π').
 Notation "π ^-1" := (@finperm_inv _ π) : finperm_scope.
-Notation "π ~" := (@can_perm_of_finPerm _ π) 
-  (at level 0) : finperm_scope.  
+Notation "π ~" := (@can_perm_of_finPerm _ π)
+  (at level 0) : finperm_scope.
 
 Section FinPermTheory.
 
 Variable (K : keyType).
-  
+
 Implicit Types (π : {finperm K}) (a : K).
 
 Lemma can_inv π : π^-1~ = π~^-1%g.
 Proof.
 apply permP => a. rewrite perm_of_finPermE.
-apply val_inj => /=. rewrite finsfun_of_can_ffunE ffunE. 
+apply val_inj => /=. rewrite finsfun_of_can_ffunE ffunE.
 suff : {| fsval := fsval a; fsvalP := fsvalP a |} = a by move ->.
 by apply val_inj.
 Qed.
 
 Lemma finperm_invK : involutive (@finperm_inv K).
 Proof.
-move => π. apply/eq_finPermP/eq1_finPermP/forallP. 
+move => π. apply/eq_finPermP/eq1_finPermP/forallP.
 rewrite fsetUid => a. rewrite !finPerm_can; do ?apply: valP.
 move => aπ ainvinvπ. rewrite val_eqE can_inv can_inv invgK.
 suff : ainvinvπ = aπ by move ->.
@@ -237,21 +237,21 @@ Qed.
 Lemma finpermVK π : cancel π^-1 π.
 Proof. by move=> a; rewrite -{1}[π]finperm_invK finpermK. Qed.
 
-Lemma finperm_invP : left_inverse (1 K) (@finperm_inv K) (@finperm_mul K).
+Lemma finperm_invP : left_inverse 1 (@finperm_inv K) (@finperm_mul K).
 Proof.
-move => π. apply/eq_finPermP => a. 
-by rewrite finsfunM /= finpermK finsfun1. 
+move => π. apply/eq_finPermP => a.
+by rewrite finsfunM /= finpermK finsfun1.
 Qed.
 
-Lemma finperm_oneP : left_id (1 K) (@finperm_mul K).
+Lemma finperm_oneP : left_id 1 (@finperm_mul K).
 Proof. move => π. apply/eq_finPermP => a. by rewrite finsfunM /= finsfun1. Qed.
 
-Lemma finperm_invVP : right_inverse (1 K) (@finperm_inv K) (@finperm_mul K).
+Lemma finperm_invVP : right_inverse 1 (@finperm_inv K) (@finperm_mul K).
 Proof. move => π. by rewrite -(finperm_invP π^-1) finperm_invK. Qed.
 
 Lemma finperm_mulA : associative (@finperm_mul K).
-Proof. 
-move => π1 π2 π3. apply/eq_finPermP => a /=. by rewrite !finsfunM /= !finsfunM. 
+Proof.
+move => π1 π2 π3. apply/eq_finPermP => a /=. by rewrite !finsfunM /= !finsfunM.
 Qed.
 
 Lemma finperm_can2eq π x y :( π x == y) = (x == π^-1 y).
@@ -261,13 +261,13 @@ End FinPermTheory.
 
 Section Transpositions.
 
-Variable (K : keyType).  
-  
+Variable (K : keyType).
+
 Implicit Types (a b c : K).
 
-Local Notation transp a b := [fun z => z with a |-> b, b |-> a].               
+Local Notation transp a b := [fun z => z with a |-> b, b |-> a].
 
-Definition tfinsfun a b := 
+Definition tfinsfun a b :=
   @finsfun_of_fun _ _ (@id K) [fun z => z with a |-> b, b |-> a] [fset a;b].
 
 CoInductive tfinperm_spec a b c : K -> Type :=
@@ -275,23 +275,23 @@ CoInductive tfinperm_spec a b c : K -> Type :=
   | TFinpermSecond of c = b : tfinperm_spec a b c a
   | TFinpermNone of (c != a) && (c != b) : tfinperm_spec a b c c.
 
-Lemma tfinpermP a b c  : 
+Lemma tfinpermP a b c  :
   tfinperm_spec a b c (tfinsfun a b c).
 Proof.
 rewrite finsfun_of_funE /=; last first.
-  move => {c} c /=. apply contraR. rewrite in_fset2 negb_or 
+  move => {c} c /=. apply contraR. rewrite in_fset2 negb_or
   => /andP [ c_neq_a c_neq_b]. by rewrite (negbTE c_neq_a) (negbTE c_neq_b).
 have [c_eq_a | c_neq_a] := (boolP (c == a)).
   by constructor; apply/eqP.
 have [c_eq_b | c_neq_b] := (boolP (c == b)).
   by constructor; apply/eqP.
-by constructor; apply /andP. 
+by constructor; apply /andP.
 Qed.
 
-Lemma inj_tfinsfun a b : 
+Lemma inj_tfinsfun a b :
   injectiveb_finsfun_id (tfinsfun a b).
-Proof. 
-apply/injectiveb_finsfunP => x y. 
+Proof.
+apply/injectiveb_finsfunP => x y.
 by case: tfinpermP; case: tfinpermP => //; do ?move-> => // ;
 move/andP => [neq1 neq2] eq1; do ?move => eq2;
 move : neq1 neq2; rewrite ?eq1 ?eq2 eqxx.
@@ -320,37 +320,37 @@ by move => zNab; rewrite tfinpermNone // andbC.
 Qed.
 
 Lemma tfinsfun_id a :
-  tfinsfun a a = (1 K).
+  tfinsfun a a = 1.
 Proof.
 apply/finsfunP => b; rewrite finsfun1.
 by case: tfinpermP; symmetry.
 Qed.
 
 Lemma tfinperm_id a :
-  tfinperm a a = (1 K).
+  tfinperm a a = 1.
 Proof.
 apply/eq_finPermP => x /=.
 by rewrite tfinsfun_id /=.
 Qed.
 
 Lemma tfinperm_idempotent a b :
-  (tfinperm a b) * (tfinperm a b) = (1 K).
+  (tfinperm a b) * (tfinperm a b) = 1.
 Proof.
 apply/eq_finPermP => c.
 rewrite finsfunM finsfun1 /=.
 case: tfinpermP; case: tfinpermP;
-  do ?(by move ->).  
-  - by move /andP => [/eqP ? /eqP ?]. 
+  do ?(by move ->).
   - by move /andP => [/eqP ? /eqP ?].
-  - by rewrite eqxx => _ /andP [? ?]. 
-  - by rewrite eqxx => _ /andP [? ?]. 
+  - by move /andP => [/eqP ? /eqP ?].
+  - by rewrite eqxx => _ /andP [? ?].
+  - by rewrite eqxx => _ /andP [? ?].
 Qed.
 
 Lemma tfinperm_conj a a' (π : {finperm K}) :
   π * (tfinperm a a') = tfinperm (π a) (π a') * π.
 Proof.
 apply/eq_finPermP => b. rewrite !finsfunM /=.
-case: (tfinpermP a a' b) ; do ?move ->; 
+case: (tfinpermP a a' b) ; do ?move ->;
 rewrite ?tfinpermL ?tfinpermR ?tfinsfun_id ?finsfun1 //.
 move/andP => [ab a'b]. have [πb_out] : (π b != π a) && (π b != π a').
   by rewrite !inj_eq; do ?apply finperm_inj; apply/andP.
@@ -368,16 +368,16 @@ Proof. by rewrite tfinperm_conj finpermVK. Qed.
 Lemma tfinperm_supp x y : finsupp (tfinperm x y) `<=` [fset x;y].
 Proof.
 apply/fsubsetP => z. rewrite mem_finsupp in_fset2.
-apply contraR => /norP /andP ?. 
+apply contraR => /norP /andP ?.
 by apply/eqP/tfinpermNone.
 Qed.
 
-Lemma tfinperm_disj x y S : 
+Lemma tfinperm_disj x y S :
   x \notin S -> y \notin S -> [disjoint S & (finsupp (tfinperm x y))].
 Proof.
 move => xNS yNS.
 rewrite fdisjoint_sym. apply (@fdisjoint_trans _ _ [fset x;y]);
-  first exact: tfinperm_supp.                       
+  first exact: tfinperm_supp.
 apply/fdisjointP => z. rewrite in_fset2 => /orP.
 by case => /eqP ->.
 Qed.
