theories/w.v
@@ -1,6 +1,6 @@
-From Ssreflect
+From mathcomp
 Require Import ssreflect ssrfun ssrbool ssrnat eqtype choice seq fintype.
-From MathComp
+From mathcomp
 Require Import finfun finset generic_quotient bigop tuple.
 
 Require Import finmap finsfun finperm nominal utilitaires.
@@ -29,9 +29,9 @@ Context (cons_label : eqType)
 
 Section WDef.
 
-Inductive rW := 
+Inductive rW :=
 |rVar of atom
-|rCons : forall (c : cons_label), 
+|rCons : forall (c : cons_label),
            cons_annot c -> ('I_(cons_arity c) -> rW) -> rW
 |rBCons : forall (c : bcons_label) (x : atom),
             bcons_annot c -> ('I_(bcons_arity c) -> rW) -> rW.
@@ -62,8 +62,8 @@ Fixpoint rW_act (π : {finperm atom}) (t : rW) :=
     |rBCons c x a f => @rBCons c (π x) a (fun i => rW_act π (f i))
   end.
 
-Lemma rW_act1 : rW_act (1 atom) =1 id.
-Proof. 
+Lemma rW_act1 : rW_act 1 =1 id.
+Proof.
 elim => [x|c a f IH|c x a f IH] /=.
   - by rewrite finsfun1.
   - congr rCons.
@@ -72,7 +72,7 @@ elim => [x|c a f IH|c x a f IH] /=.
     exact/funext/IH.
 Qed.
 
-Lemma rW_actM π π' (t : rW) : 
+Lemma rW_actM π π' (t : rW) :
   rW_act (π * π') t = rW_act π (rW_act π' t).
 Proof.
 elim : t => [x|c a f IH|c x a f IH] /=.
@@ -86,16 +86,16 @@ Qed.
 Lemma rW_actproper : forall t1 t2 π, t1 = t2 -> (rW_act π t1) = (rW_act π t2).
 Proof. by move => t1 t2 π ->. Qed.
 
-Definition rW_nominal_setoid_mixin := 
-  @PermSetoidMixin rW (@eq rW) atom rW_act rW_act1 
-                   rW_actM rW_actproper.   
+Definition rW_nominal_setoid_mixin :=
+  @PermSetoidMixin _ rW (@eq rW) rW_act rW_act1
+                   rW_actM rW_actproper.
 
 
 Fixpoint rW_support t :=
   match t with
     |rVar x => [fset x]
     |rCons c a f => \fbigcup_ (i in 'I_(cons_arity c)) (rW_support (f i))
-    |rBCons c x a f => x |` 
+    |rBCons c x a f => x |`
                        \fbigcup_(i in 'I_(bcons_arity c)) (rW_support (f i))
   end.
 
@@ -115,24 +115,24 @@ elim : t => [x|c a f IH|c x a f IH] Hsupp /=.
   - rewrite Hsupp; last exact/fset1U1.
     congr rBCons.
     apply/funext => i. apply/IH => y y_supp_fi.
-    apply/Hsupp/fsetUP; right. 
+    apply/Hsupp/fsetUP; right.
     apply/fbigcupP. by exists i.
 Qed.
 
 End WDef.
 
 Definition rW_nominal_mixin  :=
-  @NominalMixin rW_choiceType  atom rW_nominal_setoid_mixin _ 
+  @NominalMixin _ rW_choiceType rW_nominal_setoid_mixin _
                 rW_act_id.
 
-Canonical rW_nominalType := 
-  @NominalType atom rW_choiceType rW_nominal_mixin.
+Canonical rW_nominalType :=
+  NominalType atom rW rW_nominal_mixin.
 
 Section rDepth.
-  
-Lemma rdepth_perm (π : {finperm atom}) (t : rW) : 
+
+Lemma rdepth_perm (π : {finperm atom}) (t : rW) :
 rW_depth (π \dot t) = rW_depth t.
-Proof. 
+Proof.
 elim : t => [x|c a f IH|c x a f IH] //;
 exact/eq_S/eq_big.
 Qed.
@@ -144,51 +144,51 @@ Section AlphaEquivalence.
 Fixpoint alpha_rec (n : nat) (W1 W2 : rW ) :=
   match n, W1, W2 with
     |_, rVar x, rVar y => x == y
-    |S n, rCons c1 a1 f1, rCons c2 a2 f2 => 
+    |S n, rCons c1 a1 f1, rCons c2 a2 f2 =>
      match (eq_comparable c1 c2) with
-       |left p => (eq_rect c1 
-                  (fun c => forall (a2 : cons_annot c) 
-                                   (f2 : 'I_(cons_arity c) -> rW), bool) 
-                  (fun a2 f2 => 
-                     (a1 == a2) && 
+       |left p => (eq_rect c1
+                  (fun c => forall (a2 : cons_annot c)
+                                   (f2 : 'I_(cons_arity c) -> rW), bool)
+                  (fun a2 f2 =>
+                     (a1 == a2) &&
                      [forall i in 'I_(cons_arity c1), alpha_rec n (f1 i) (f2 i)]) c2 p)
                     a2 f2
        |right _ => false
      end
     |S n, rBCons c1 x1 a1 f1, rBCons c2 x2 a2 f2 =>
      match (eq_comparable c1 c2) with
-       |left p => 
+       |left p =>
         (eq_rect c1
-                 (fun c => 
-                    forall 
+                 (fun c =>
+                    forall
                       (x2 : atom)
                       (a2 : bcons_annot c)
                       (f2 : 'I_(bcons_arity c) -> rW), bool)
                  (fun x2 a2 f2 =>
-                    (a1 == a2) && 
+                    (a1 == a2) &&
                      let m := bcons_arity c1 in
                      let z := fresh_in (x1, x2, f1, f2) in
                      [forall i in 'I_m, alpha_rec n (swap x1 z \dot f1 i)
                                                     (swap x2 z \dot f2 i)]) c2 p)
-          x2 a2 f2                            
+          x2 a2 f2
        |right _ => false
      end
     |_, _,_ => false
   end.
 
-Definition alpha W1 W2 := alpha_rec (rW_depth W1) W1 W2.     
+Definition alpha W1 W2 := alpha_rec (rW_depth W1) W1 W2.
 
-Lemma alpha_recE n (W1 W2 : rW) : 
-  (rW_depth W1 <= n) -> 
+Lemma alpha_recE n (W1 W2 : rW) :
+  (rW_depth W1 <= n) ->
   alpha_rec n W1 W2 = alpha W1 W2.
 Proof.
-rewrite /alpha; move: {-2}n (leqnn n). 
+rewrite /alpha; move: {-2}n (leqnn n).
 elim: n W1 W2 => // [|n ihn] [x1|c1 a1 f1|c1 x1 a1 f1] [x2|c2 a2 f2|c2 x2 a2 f2] [|m] //.
-all: rewrite ltnS => m_leq_n IHf1 /=. 
-all: case: (eq_comparable c1 c2) => // p. 
-all: destruct p => /=; apply andb_id2l => _. 
-all: apply eq_forallb => i. 
-all: rewrite !ihn // ?rdepth_perm; 
+all: rewrite ltnS => m_leq_n IHf1 /=.
+all: case: (eq_comparable c1 c2) => // p.
+all: destruct p => /=; apply andb_id2l => _.
+all: apply eq_forallb => i.
+all: rewrite !ihn // ?rdepth_perm;
   first exact/(@leq_trans m); first exact/leq_bigmax.
 all: move: IHf1 => /bigmax_leqP /(_ i); exact.
 Qed.
@@ -198,25 +198,26 @@ Lemma alpha_equivariant (W1 W2 : rW ) (π : {finperm atom}):
 Proof.
 rewrite/alpha rdepth_perm.
 move: {-1}(rW_depth W1) (leqnn (rW_depth W1)) => n.
-elim: n W1 W2 π => [|n IHn] [x1|c1 a1 f1|c1 x1 a1 f1] 
+elim: n W1 W2 π => [|n IHn] [x1|c1 a1 f1|c1 x1 a1 f1]
                             [x2|c2 a2 f2|c2 x2 a2 f2] π //=;
-  try solve [rewrite inj_eq //; exact: act_inj].
+  do ?by rewrite inj_eq //; apply/finperm_inj.
 all: rewrite ltnS => /bigmax_leqP IHl1.
 all: case: (eq_comparable c1 c2) => p //; destruct p => /=.
-all: apply andb_id2l => _. 
+all: apply andb_id2l => _.
 all: apply eq_forallb => i.
   exact/IHn/IHl1.
 set z := fresh_in _; set y := fresh_in _.
 rewrite -act_conj_imL -[X in alpha_rec _ _ X]act_conj_imL.
 rewrite IHn; try rewrite -[RHS](@IHn _ _ (swap y (π^-1 z)));
-  try solve [rewrite rdepth_perm; exact: IHl1]. 
-freshTacCtxt z; freshTacCtxt y.
-rewrite -{1}[f1 i](@act_fresh _ y (π^-1 z)) //; 
-  [|exact/fresh_fun|exact/fresh_fun/im_inv_fresh]. 
-rewrite -{1}[f2 i](@act_fresh _ y (π^-1 z)) //; 
-  [|exact/fresh_fun|exact/fresh_fun/im_inv_fresh]. 
-rewrite 2?[in RHS]act_conj tfinpermL !tfinperm_fresh //.
-all: exact/im_inv_fresh. 
+  try solve [rewrite rdepth_perm; exact: IHl1].
+freshTacCtxt y.
+freshTacCtxt z.
+rewrite -{1}[f1 i](@act_fresh _ y (π^-1 z)) //;
+  [|exact/fresh_fun|exact/fresh_fun/im_inv_fresh].
+rewrite -{1}[f2 i](@act_fresh _ y (π^-1 z)) //;
+  [|exact/fresh_fun|exact/fresh_fun/im_inv_fresh].
+do ?rewrite [swap y _ \dot _  \dot _]act_conj tfinpermL tfinperm_fresh //;
+   do?exact/im_inv_fresh.
 Qed.
 
 Lemma alpha_equivariantprop : equivariant_prop alpha.
@@ -231,7 +232,7 @@ Lemma alpha_Cons_eqc (c1 c2 : cons_label) a1 a2 f1 f2 :
 Proof. rewrite/alpha/=; by case: (eq_comparable c1 c2). Qed.
 
 Lemma alpha_ConsP (c : cons_label) (a1 a2 : cons_annot c) f1 f2 :
-  reflect (a1 = a2 /\ forall i, alpha (f1 i) (f2 i)) 
+  reflect (a1 = a2 /\ forall i, alpha (f1 i) (f2 i))
           (alpha (@rCons c a1 f1) (@rCons c a2 f2)).
 Proof.
 rewrite/alpha /=.
@@ -246,7 +247,7 @@ apply: (iffP idP).
 move => [->] H; rewrite eqxx /=.
 apply/forallP => i /=.
 rewrite alpha_recE; first exact/H.
-exact/(@leq_bigmax _ (fun i => rW_depth (f1 i))). 
+exact/(@leq_bigmax _ (fun i => rW_depth (f1 i))).
 Qed.
 
 Lemma alpha_BCons_eqc (c1 c2 : bcons_label) x1 x2 a1 a2 f1 f2 :
@@ -254,7 +255,7 @@ Lemma alpha_BCons_eqc (c1 c2 : bcons_label) x1 x2 a1 a2 f1 f2 :
 Proof. rewrite/alpha/=; by case: (eq_comparable c1 c2). Qed.
 
 Lemma alpha_BConsE (c : bcons_label) (x1 x2 : atom) a1 a2 f1 f2 :
-  alpha (@rBCons c x1 a1 f1) (@rBCons c x2 a2 f2) = 
+  alpha (@rBCons c x1 a1 f1) (@rBCons c x2 a2 f2) =
   (a1 == a2) && let z := fresh_in (x1, x2, f1, f2) in
                 [forall i, alpha (swap x1 z \dot (f1 i)) (swap x2 z \dot (f2 i))].
 Proof.
@@ -264,11 +265,11 @@ have -> /= : p = erefl c by apply eq_axiomK.
 apply/andb_id2l => _.
 apply/eq_forallb => i.
 rewrite alpha_recE // rdepth_perm.
-exact/(@leq_bigmax _ (fun i => rW_depth (f1 i))). 
+exact/(@leq_bigmax _ (fun i => rW_depth (f1 i))).
 Qed.
 
 Lemma alpha_BConsP (c : bcons_label) (x1 x2 : atom) a1 a2 f1 f2  :
-  reflect (a1 = a2 /\ 
+  reflect (a1 = a2 /\
            let n := bcons_arity c in
            \new z, (forall i, alpha (swap x1 z \dot (f1 i)) (swap x2 z \dot (f2 i))))
           (alpha (@rBCons c x1 a1 f1) (@rBCons c x2 a2 f2)).
@@ -277,14 +278,14 @@ move : (equi_funprop (@swap_equiv _) alpha_equivariantprop) => /= Requi.
 rewrite /alpha /=.
 case: (eq_comparable c c) => p //.
 have -> /= : p = erefl c by apply eq_axiomK.
-set z := fresh_in _. 
+set z := fresh_in _.
 apply: (equivP andP); apply and_iff_congr => /=.
   by symmetry; apply (rwP eqP).
 eapply iff_stepl. by symmetry; apply/new_all.
 eapply iff_stepl. exact/(rwP forallP).
 apply forall_iff => i.
-rewrite alpha_recE ?rdepth_perm; 
-  last exact/(@leq_bigmax _ (fun i => rW_depth (f1 i))). 
+rewrite alpha_recE ?rdepth_perm;
+  last exact/(@leq_bigmax _ (fun i => rW_depth (f1 i))).
 apply (@some_fresh_new _ _ Requi _ ((x1, f1 i), (x2, f2 i))).
 freshTacCtxt z.
 repeat (apply/fresh_prod; split) => //.
@@ -293,7 +294,7 @@ Qed.
 
 Lemma alpha_refl : reflexive alpha.
 Proof.
-elim => [x|c a f IH|c x a f IH]. 
+elim => [x|c a f IH|c x a f IH].
   - exact/alpha_VarP.
   - by apply/alpha_ConsP; split.
   - rewrite alpha_BConsE eqxx /=.
@@ -307,8 +308,8 @@ move => t1 t2; rewrite/alpha.
 move: {-1}(rW_depth t1) (leqnn (rW_depth t1)) => n.
 elim: n t1 t2 => [|n IHn] [x1|c1 a1 f1|c1 x1 a1 f1] [x2|c2 a2 f2|c2 x2 a2 f2] //=.
 all: rewrite ltnS => /bigmax_leqP depth_f1_leqn.
-all: case: (eq_comparable c1 c2) => p. 
-all: case: (eq_comparable c2 c1) => q. 
+all: case: (eq_comparable c1 c2) => p.
+all: case: (eq_comparable c2 c1) => q.
 all: try congruence.
 all: have -> : q = sym_eq p by exact/eq_irrelevance.
 all: destruct p => /=; rewrite eq_sym; apply andb_id2l => _.
@@ -326,8 +327,8 @@ Qed.
 Lemma alpha_trans : transitive alpha.
 move => t2 t1 t3.
 move: {-1}(rW_depth t1) (leqnn (rW_depth t1)) => n.
-elim: n t1 t2 t3 => [|n IHn] [x1|c1 a1 f1|c1 x1 a1 f1] 
-                             [x2|c2 a2 f2|c2 x2 a2 f2] 
+elim: n t1 t2 t3 => [|n IHn] [x1|c1 a1 f1|c1 x1 a1 f1]
+                             [x2|c2 a2 f2|c2 x2 a2 f2]
                              [x3|c3 a3 f3|c3 x3 a3 f3] //=;
 try solve [move => _; apply eq_op_trans].
 all: rewrite ltnS => /bigmax_leqP depthf1_leqn.
@@ -354,8 +355,8 @@ End AlphaEquivalence.
 
 Section Quotient.
 
-Canonical alpha_equiv := 
-  EquivRel alpha alpha_refl alpha_sym alpha_trans. 
+Canonical alpha_equiv :=
+  EquivRel alpha alpha_refl alpha_sym alpha_trans.
 
 Definition W := {eq_quot alpha}.
 Definition W_eqMixin := [eqMixin of W].
@@ -363,7 +364,7 @@ Canonical W_eqType := EqType W W_eqMixin.
 Canonical W_choiceType := Eval hnf in [choiceType of W].
 Canonical W_countType := Eval hnf in [countType of W].
 Canonical W_quotType := Eval hnf in [quotType of W].
-Canonical W_eqQuotType := Eval hnf in 
+Canonical W_eqQuotType := Eval hnf in
       [eqQuotType alpha of W].
 
 Lemma alpha_eqE t t' : alpha t t' = (t == t' %[mod W]).
@@ -379,13 +380,13 @@ Definition Var x := lift_cst W (rVar x).
 Lemma rVarK x : \pi_W (rVar x) = Var x.
 Proof. by unlock Var. Qed.
 
-Notation lift_fun cons := 
+Notation lift_fun cons :=
   (locked (fun f => \pi_W (cons (fun i => (@repr _ W_quotType (f i)))))).
 
 Definition Cons c a := lift_fun (@rCons c a).
 Lemma rConsK c a f : \pi_W (@rCons c a f) = @Cons c a (\pi \o f).
 Proof.
-unlock Cons; apply/eqP. 
+unlock Cons; apply/eqP.
 rewrite [_ == _]piE. apply/alpha_ConsP; split => // i.
 by rewrite alpha_eqE reprK.
 Qed.
@@ -394,7 +395,7 @@ Definition BCons c x a := lift_fun (@rBCons c x a).
 Lemma rBConsK c x a f : \pi_W (@rBCons c x a f) = @BCons c x a (\pi \o f).
 Proof.
 unlock BCons; apply/eqP.
-rewrite [_ == _]piE alpha_BConsE eqxx /=. 
+rewrite [_ == _]piE alpha_BConsE eqxx /=.
 apply/forallP => i.
 by rewrite alpha_equivariant alpha_eqE reprK.
 Qed.
@@ -407,61 +408,61 @@ Implicit Types (π : {finperm atom}).
 
 Definition W_act π (t : W) := \pi_W (π \dot repr t).
 
-Lemma W_act1 : W_act (1 atom) =1 id.
+Lemma W_act1 : W_act 1 =1 id.
 Proof. move => t /=. by rewrite /W_act act1 reprK. Qed.
 
-Lemma W_act_equiv π t : 
-  π \dot (repr t) == repr (W_act π t) %[mod W].   
+Lemma W_act_equiv π t :
+  π \dot (repr t) == repr (W_act π t) %[mod W].
 Proof. by rewrite /W_act reprK. Qed.
 
 Lemma W_actM π π' t : W_act (π * π') t = W_act π (W_act π' t).
 Proof.
-apply/eqP. 
-by rewrite /W_act actM piE alpha_equivariant alpha_eqE reprK. 
+apply/eqP.
+by rewrite /W_act actM piE alpha_equivariant alpha_eqE reprK.
 Qed.
 
-Lemma W_actproper : 
+Lemma W_actproper :
   forall t1 t2 π, t1 = t2 -> (W_act π t1) = (W_act π t2).
 Proof. by move => t1 t2 π ->. Qed.
 
 Definition W_nominal_setoid_mixin :=
-  @PermSetoidMixin W (@eq W) atom W_act W_act1 W_actM W_actproper.
+  @PermSetoidMixin _ W (@eq W) W_act W_act1 W_actM W_actproper.
 
 Lemma W_act_id π t :
-     (forall a : atom, a \in rW_support (repr t) -> π a = a) -> 
+     (forall a : atom, a \in rW_support (repr t) -> π a = a) ->
      W_act π t = t.
 Proof.
 rewrite/W_act => Hact_id.
-by rewrite act_id // reprK. 
+by rewrite act_id // reprK.
 Qed.
 
 Definition W_nominal_mixin :=
-  @NominalMixin W_choiceType atom W_nominal_setoid_mixin _ W_act_id.
+  @NominalMixin _ _ W_nominal_setoid_mixin _ W_act_id.
 
-Canonical W_nominalType := @NominalType atom W_choiceType W_nominal_mixin.
+Canonical W_nominalType := NominalType atom W W_nominal_mixin.
 
 End NominalW.
 
 Section VariousLemmas.
 
-Lemma pi_equivariant π (t : rW) : 
+Lemma pi_equivariant π (t : rW) :
   π \dot (\pi_W t) = \pi_W (π \dot t).
 Proof.
-apply/eqmodP => /=. 
-by rewrite alpha_equivariant alpha_eqE reprK. 
+apply/eqmodP => /=.
+by rewrite alpha_equivariant alpha_eqE reprK.
 Qed.
 
-Lemma repr_equivariant π (t : W) : repr (π \dot t) == π \dot (repr t) %[mod W]. 
+Lemma repr_equivariant π (t : W) : repr (π \dot t) == π \dot (repr t) %[mod W].
 Proof. by rewrite -pi_equivariant !reprK. Qed.
 
 Lemma Var_equivariant π x : π \dot (Var x) = Var (π x).
 Proof. by rewrite -rVarK pi_equivariant /= rVarK. Qed.
 
-Lemma Cons_equivariant π c a f : 
+Lemma Cons_equivariant π c a f :
   π \dot (@Cons c a f) = @Cons c a (π \dot f).
 Proof.
-unlock Cons. 
-rewrite pi_equivariant !rConsK. 
+unlock Cons.
+rewrite pi_equivariant !rConsK.
 congr Cons.
 apply/funext => i /=.
 exact/sym_eq/eqP/repr_equivariant.
@@ -470,7 +471,7 @@ Qed.
 Lemma BCons_equivariant π c x a f :
   π \dot (@BCons c x a f) = @BCons c (π x) a (π \dot f).
 Proof.
-unlock BCons. 
+unlock BCons.
 rewrite pi_equivariant !rBConsK.
 congr BCons.
 apply/funext => i /=.
@@ -491,7 +492,7 @@ exists S; split => //.
 move => π H. by rewrite pi_equivariant (S_supp_t π).
 Qed.
 
-Lemma fresh_fun_pi {I : finType} x (f : I -> rW) : 
+Lemma fresh_fun_pi {I : finType} x (f : I -> rW) :
   x # f -> x # (\pi_W \o f).
 Proof.
 move => xF.
@@ -509,7 +510,7 @@ Lemma eq_BConsE c x1 x2 a1 a2 f1 f2 :
              swap x1 z \dot f1 = swap x2 z \dot f2.
 Proof.
 unlock BCons => /eqP.
-rewrite -alpha_eqE alpha_BConsE => /andP [/eqP ->] /=. 
+rewrite -alpha_eqE alpha_BConsE => /andP [/eqP ->] /=.
 set z := fresh_in _ => /forallP Halpha.
 split => // z'.
 repeat(move/fresh_prod; case); move => *.
@@ -523,18 +524,18 @@ rewrite ![swap z z' \dot _]act_fresh.
 all:exact/fresh_fun.
 Qed.
 
-Lemma VarK x : repr (Var x) = rVar x. 
+Lemma VarK x : repr (Var x) = rVar x.
 Proof.
-have : alpha (repr (Var x)) (rVar x). 
-  by rewrite alpha_eqE reprK rVarK. 
-by case: (repr (Var x)) => // ? /eqP ->. 
+have : alpha (repr (Var x)) (rVar x).
+  by rewrite alpha_eqE reprK rVarK.
+by case: (repr (Var x)) => // ? /eqP ->.
 Qed.
 
 Lemma ConsK c a f  : exists f', repr (@Cons c a f) = @rCons c a f' /\ (f = \pi \o f').
 Proof.
 have: alpha (repr (@Cons c a f)) (@rCons c a (repr \o f)).
-  by rewrite alpha_eqE reprK rConsK pi_reprK. 
-case: (repr (Cons _ _)) => //= c2 a2 f2. 
+  by rewrite alpha_eqE reprK rConsK pi_reprK.
+case: (repr (Cons _ _)) => //= c2 a2 f2.
 have [/eqP c_eq_c2|/eqP c_neq_c2 /alpha_Cons_eqc] := boolP (c == c2);
     last by congruence.
 subst.
@@ -549,8 +550,8 @@ Lemma BConsK c x a f : exists (y : atom) f',
    repr (@BCons c x a f) = @rBCons c y a f'.
 Proof.
 have: alpha (repr (@BCons c x a f)) (@rBCons c x a (repr \o f)).
-  by rewrite alpha_eqE reprK rBConsK pi_reprK.  
-case: (repr (BCons _ _ _)) => //= c2 x2 a2 f2. 
+  by rewrite alpha_eqE reprK rBConsK pi_reprK.
+case: (repr (BCons _ _ _)) => //= c2 x2 a2 f2.
 have [/eqP c_eq_c2|/eqP c_neq_c2 /alpha_BCons_eqc] := boolP (c == c2);
     last by congruence.
 subst.
@@ -561,7 +562,7 @@ Qed.
 
 
 Lemma Var_inj : injective Var.
-Proof. 
+Proof.
 move => x y /(congr1 repr). rewrite !VarK => H. by injection H. Qed.
 
 Lemma Cons_inj c a1 a2 f1 f2 :
@@ -578,7 +579,7 @@ have -> /= : q = erefl c by apply/eq_axiomK.
 by [].
 Qed.
 
-Lemma BConsx_inj c x a1 a2 f1 f2 : 
+Lemma BConsx_inj c x a1 a2 f1 f2 :
   (@BCons c x a1 f1 = @BCons c x a2 f2) -> a1 = a2 /\ f1 = f2.
 Proof.
 pose z := fresh_in (x, f1, f2).
@@ -610,11 +611,11 @@ Lemma fresh_rBCons x y c a f :
 Proof.
 move => [S] [xNS S_supp_cyl].
 exists S; split => // π Hπ.
-move: (S_supp_cyl π Hπ) => H.  injection H. 
-move => /eq_sigT_sig_eq [p]. 
+move: (S_supp_cyl π Hπ) => H.  injection H.
+move => /eq_sigT_sig_eq [p].
 have -> /= : p = erefl c by apply eq_axiomK.
 move => πf_eq_f.
-by rewrite prodactE atomactE -{2}πf_eq_f => ->. 
+by rewrite prodactE atomactE -{2}πf_eq_f => ->.
 Qed.
 
 Lemma fresh_BCons x y c a f :
@@ -623,7 +624,7 @@ Proof.
 move => [S] [xNS S_supp_y] [S'] [xNS' S'_supp_cyf].
 exists (S `|` S'); split.
   by rewrite in_fsetU negb_or xNS xNS'.
-move => π Hπ. 
+move => π Hπ.
 apply/(proj2 (@BConsx_inj c y a a _ _ _)).
 have y_eq_piy : π y = y.
   apply S_supp_y => b bS. apply Hπ.
@@ -632,13 +633,13 @@ rewrite -{1}y_eq_piy -BCons_equivariant.
 apply S'_supp_cyf => b bS'. apply Hπ.
 by rewrite in_fsetU bS' orbT.
 Qed.
-  
+
 Lemma eq_BCons c x y a f :
   y # (x, f) -> @BCons c x a f = @BCons c y a (swap x y \dot f).
 Proof.
 repeat(move/fresh_prod; case); move => yFx yFf.
-unlock BCons. apply/eqmodP. 
-rewrite /= alpha_BConsE eqxx /=. 
+unlock BCons. apply/eqmodP.
+rewrite /= alpha_BConsE eqxx /=.
 apply/forallP => i.
 rewrite alpha_eqE -!pi_equivariant !reprK.
 set z := fresh_in _. freshTacCtxt z.
@@ -648,11 +649,11 @@ apply/fresh_repr. change (z # ((repr \o f) i)).
 exact/fresh_fun.
 Qed.
 
-Lemma bname_fresh x c a f : x # (@BCons c x a f).
+Lemma bname_fresh (x : atom) c a f : x # (@BCons c x a f).
 Proof.
 pose y := fresh_in (x, f, @BCons c x a f); freshTacCtxt y.
 apply (@CFN_principle y) => //.
-rewrite BCons_equivariant tfinpermL. 
+rewrite BCons_equivariant tfinpermL.
 exact/sym_eq/eq_BCons/fresh_prod.
 Qed.
 
@@ -662,24 +663,24 @@ Section Depth.
 
 Definition depth (t : W) := rW_depth (repr t).
 
-Lemma rdepth_alpha t u : alpha t u -> rW_depth t = rW_depth u. 
+Lemma rdepth_alpha t u : alpha t u -> rW_depth t = rW_depth u.
 Proof.
 elim: t u => [x1|c1 a1 f1 IHf1|c1 x1 a1 f1 IHf1] [x2|c2 a2 f2|c2 x2 a2 f2] //=.
 all: have [/eqP c1_eq_c2|/eqP c1_neq_c2] := boolP (c1 == c2).
   2: by move/alpha_Cons_eqc; congruence.
-  3: by move/alpha_BCons_eqc; congruence.  
+  3: by move/alpha_BCons_eqc; congruence.
 all: subst.
 1: move/alpha_ConsP => [_ alpha_f1_f2].
 2: rewrite alpha_BConsE; set z := fresh_in _  => /andP [_ /= /forallP alpha_f1_f2].
-all: apply/eq_S/eq_bigr => i _. 
+all: apply/eq_S/eq_bigr => i _.
   exact/IHf1.
 move: (alpha_f1_f2 i).
 rewrite -(alpha_equivariant _ _ (swap x1 z)) -actM tfinperm_idempotent act1 => /IHf1.
 by rewrite !rdepth_perm.
 Qed.
-                                                     
+
 Lemma depth_rdepth t : depth (\pi t) = rW_depth t.
-Proof. 
+Proof.
 apply rdepth_alpha. by rewrite alpha_eqE reprK.
 Qed.
 
@@ -696,7 +697,7 @@ Proof. by rewrite/depth VarK. Qed.
 Lemma depth_Cons c a f : depth (@Cons c a f) = (\max_i (depth (f i))).+1.
 Proof. unlock Cons. by rewrite depth_rdepth /=. Qed.
 
-Lemma depth_BinderCons c x a f : 
+Lemma depth_BinderCons c x a f :
   depth (@BCons c x a f) = (\max_i (depth (f i))).+1.
 Proof. unlock BCons. by rewrite depth_rdepth /=. Qed.
 
@@ -709,60 +710,60 @@ Lemma W_naive_ind (P : W -> Prop) :
   (forall c a f, (forall i, P (f i)) -> P (@Cons c a f)) ->
   (forall c x a f, (forall i, P (f i)) -> P (@BCons c x a f)) ->
   forall u, P u.
-Proof. 
+Proof.
 move => HVar HCons HBCons u; rewrite -[u]reprK.
 elim: (repr u) => [x|c a f IHf|c x a f IHf] /=.
-  - by rewrite rVarK.              
+  - by rewrite rVarK.
   - rewrite rConsK. exact/HCons.
   - rewrite rBConsK. exact/HBCons.
 Qed.
 
-Lemma W_ind {env : nominalType atom} (C : env) (P : W -> Prop) :
-  (forall x, P (Var x)) ->
+Lemma W_ind {env : {nominalType atom}} (C : env) (P : W -> Prop) :
+  (forall (x : atom), P (Var x)) ->
   (forall c a f, (forall i, P (f i)) -> P (@Cons c a f)) ->
   (forall c x a f, x # C -> (forall i, P (f i)) -> P (@BCons c x a f)) ->
   forall u, P u.
-Proof. 
+Proof.
 move => HVar HCons HBcons u.
 suff : forall π, P (π \dot u).
-  by move => /(_ (1 atom)); rewrite act1.
+  by move => /(_ 1); rewrite act1.
 elim/W_naive_ind : u => [x|c a f IHf|c x a f IHf] π.
   - by rewrite Var_equivariant.
-  - rewrite Cons_equivariant. apply/HCons => i. 
-    by rewrite ffunactE. 
-  - rewrite BCons_equivariant. 
-    pose z := fresh_in (C, π x, π \dot f); freshTacCtxt z.
+  - rewrite Cons_equivariant. apply/HCons => i.
+    by rewrite ffunactE.
+  - rewrite BCons_equivariant.
+    pose z := fresh_in (C, π \dot x, π \dot f); freshTacCtxt z.
     rewrite (@eq_BCons _ _ z) -?actM => //; last exact/fresh_prod.
     apply HBcons => // i.
-    by rewrite ffunactE. 
+    by rewrite ffunactE.
 Qed.
 
-Context (X : nominalType atom)
+Context (X : {nominalType atom})
         (f_var : atom -> X)
-        (f_cons : forall (c : cons_label), (cons_annot c) -> 
-                                           ('I_(cons_arity c) -> W) -> 
+        (f_cons : forall (c : cons_label), (cons_annot c) ->
+                                           ('I_(cons_arity c) -> W) ->
                                            ('I_(cons_arity c) -> X) -> X)
-        (f_bcons : forall (c : bcons_label), atom -> 
+        (f_bcons : forall (c : bcons_label), atom ->
                                              (bcons_annot c) ->
-                                             ('I_(bcons_arity c) -> W) -> 
+                                             ('I_(bcons_arity c) -> W) ->
                                              ('I_(bcons_arity c) -> X) -> X)
         (Supp : {fset atom})
         (dflt : X).
 
-Hypothesis f_var_equivariant : 
-  forall (π : {finperm atom}) x, 
+Hypothesis f_var_equivariant :
+  forall (π : {finperm atom}) x,
     [disjoint finsupp π & Supp] -> π \dot f_var x = f_var (π \dot x).
 
 Hypothesis f_cons_equivariant :
   forall (π : {finperm atom}) c a f f',
     [disjoint finsupp π & Supp] ->
-                  π \dot @f_cons c a f f' = 
+                  π \dot @f_cons c a f f' =
                   @f_cons c a (π \dot f) (π \dot f').
 
 Hypothesis f_bcons_equivariant :
-  forall (π : {finperm atom}) c x a f f', 
-    [disjoint finsupp π & Supp] -> π \dot @f_bcons c x a f f' = 
-                                   @f_bcons c (π x) a (π \dot f) (π \dot f').                 
+  forall (π : {finperm atom}) c x a f f',
+    [disjoint finsupp π & Supp] -> π \dot @f_bcons c x a f f' =
+                                   @f_bcons c (π x) a (π \dot f) (π \dot f').
 
 Hypothesis FCB_fbcons :
   forall x c a f f', x # Supp -> x # (@f_bcons c x a f f').
@@ -785,7 +786,7 @@ Definition W_rect t := W_rect_rec (depth t) t.
 Lemma W_rect_recE n t : depth t <= n -> W_rect_rec n t = W_rect t.
 Proof.
 rewrite/W_rect; move: {-2}n (leqnn n).
-elim: n t => [|n IHn] t //; rewrite /depth. 
+elim: n t => [|n IHn] t //; rewrite /depth.
   by move => ?; do 2?(rewrite leqn0 => /eqP ->).
 move => [?|m]; first by rewrite leqn0 => /eqP ->.
 rewrite ltnS => m_leq_n.
@@ -796,27 +797,27 @@ all: rewrite IHn // ?depth_perm ?depth_rdepth; last exact/IHf.
 all: rewrite [RHS]IHn; first by rewrite ?depth_perm depth_rdepth.
 1: apply/(@leq_trans m) => //; exact/bigmax_leqP.
 2: apply/(@leq_trans m) => //; exact/bigmax_leqP. (* factorisation ?*)
-all: rewrite ?depth_perm depth_rdepth. 
+all: rewrite ?depth_perm depth_rdepth.
 all: exact/leq_bigmax_cond.
 Qed.
 
 Lemma W_rect_VarE x : W_rect (Var x) = f_var x.
 Proof. by rewrite /W_rect depth_Var /= VarK. Qed.
 
-Lemma W_rect_ConsE c a f : 
+Lemma W_rect_ConsE c a f :
   W_rect (@Cons c a f) = @f_cons c a f (W_rect \o f).
 Proof.
 rewrite/W_rect depth_Cons /=.
 have [f' [-> ->]] := @ConsK c a f.
 congr f_cons => //.
 apply/funext => i /=.
-apply W_rect_recE => /=. 
+apply W_rect_recE => /=.
 exact/leq_bigmax_cond.
 Qed.
 
 Lemma W_rect_BConsE_subproof c x a f :
   let z := (fresh_in (Supp, repr (@BCons c x a f))) in
-    W_rect (@BCons c x a f) = 
+    W_rect (@BCons c x a f) =
     @f_bcons c z a (swap x z \dot f) (W_rect \o (swap x z \dot f)).
 have [y [f'] repr_cxf] := @BConsK c x a f => /=.
 rewrite /W_rect depth_BinderCons /= repr_cxf.
@@ -843,27 +844,27 @@ apply/fresh_repr. rewrite repr_cxf.
 by freshTac.
 Qed.
 
-Definition equiv t := 
+Definition equiv t :=
   forall (π : {finperm atom}), [disjoint finsupp π & Supp] ->
-                               π \dot (W_rect t) = 
+                               π \dot (W_rect t) =
                                W_rect (π \dot t).
 
 Definition res c x a f := W_rect (@BCons c x a f) =
                         @f_bcons c x a f (W_rect \o f).
 
-Lemma equiv_res_subproof c x a f :
+Lemma equiv_res_subproof c (x : atom) a f :
 (forall i, equiv (f i)) ->
 x # Supp -> @res c x a f.
 Proof.
 move => Hequiv xFSupp.
 rewrite /res W_rect_BConsE_subproof; set y := fresh_in _.
 set rhs := RHS; set lhs := LHS; rewrite /lhs/rhs.
-set b := fresh_in (lhs, rhs, Supp, f, x). 
+set b := fresh_in (lhs, rhs, Supp, f, x).
 freshTacCtxt b. freshTacCtxt y.
 rewrite -[LHS](@act_fresh _ y b) //; last exact/FCB_fbcons.
 rewrite -[RHS](@act_fresh _ x b) //; last exact/FCB_fbcons.
 rewrite !f_bcons_equivariant;
-  try solve [exact/disjoint_tfsupp]. 
+  try solve [exact/disjoint_tfsupp].
 rewrite !tfinpermL.
 have : y # @BCons c x a f by apply/fresh_repr.
 have [/eqP ->|/fresh_atomP zFx /(fresh_BCons zFx) ?] := boolP (y == x).
@@ -874,7 +875,7 @@ congr f_bcons.
 apply/funext => i /=.
 rewrite !ffunactE /= -Hequiv; last exact/disjoint_tfsupp.
 rewrite act_conj tfinpermL tfinperm_fresh //.
-rewrite Hequiv; last exact/disjoint_tfsupp. 
+rewrite Hequiv; last exact/disjoint_tfsupp.
 rewrite [swap y b \dot _]act_fresh //.
 all: exact/fresh_fun.
 Qed.
@@ -884,28 +885,28 @@ Lemma W_rect_equivariant t :
 Proof.
 elim/(@W_ind _ Supp): t => [v|c a f IHf|c z a f zFSupp IHf] π disj_pi_S.
   - by rewrite Var_equivariant !W_rect_VarE f_var_equivariant.
-  - rewrite !Cons_equivariant !W_rect_ConsE f_cons_equivariant //. 
+  - rewrite !Cons_equivariant !W_rect_ConsE f_cons_equivariant //.
     congr f_cons.
     apply/funext => i.
-    by rewrite !ffunactE /= IHf . 
+    by rewrite !ffunactE /= IHf .
   - have Hres1 := (@equiv_res_subproof c _ _ _ IHf zFSupp).
     have Hres2 : @res c (π z) a (π \dot f).
-      apply/equiv_res_subproof => //; last exact/disj_im_fresh. 
+      apply/equiv_res_subproof => //; last exact/disj_im_fresh.
       move => i π' ? /=.
       rewrite -actM -!IHf // ?actM //; exact/disjoint_conj.
-    rewrite BCons_equivariant Hres1 Hres2. 
-    rewrite f_bcons_equivariant //. 
+    rewrite BCons_equivariant Hres1 Hres2.
+    rewrite f_bcons_equivariant //.
     congr f_bcons.
     apply/funext => i /=.
     by rewrite ffunactE IHf.
 Qed.
 
-Lemma W_rect_BConsE c x a f : 
-  x # Supp -> 
+Lemma W_rect_BConsE c x a f :
+  x # Supp ->
   W_rect (@BCons c x a f) = @f_bcons c x a f (W_rect \o f).
 Proof.
 move => xFsupp.
-apply/equiv_res_subproof => // ? ?. 
+apply/equiv_res_subproof => // ? ?.
 exact/W_rect_equivariant.
 Qed.
 
@@ -927,28 +928,28 @@ Definition wsubst_bcons (c : bcons_label) (y : atom) a
            (f : 'I_(bcons_arity c) -> W) res :=
   @BCons c y a res.
 
-Definition wsubst := 
+Definition wsubst :=
   @W_rect _ wsubst_var wsubst_cons wsubst_bcons Supp dflt.
 
-Lemma wsubst_var_equiv (π : {finperm atom}) y : 
-  [disjoint finsupp π & Supp] -> 
-  π \dot wsubst_var y = wsubst_var (π y). 
+Lemma wsubst_var_equiv (π : {finperm atom}) y :
+  [disjoint finsupp π & Supp] ->
+  π \dot wsubst_var y = wsubst_var (π y).
 Proof.
 rewrite fdisjoint_sym fdisjointU1X => /andP [/finsfun_dflt pix_x disj_pi_Supp].
 rewrite /wsubst_var if_equivariant -{2}pix_x (inj_eq (@finperm_inj _ π)).
 by rewrite fresh_perm // Var_equivariant.
 Qed.
-  
+
 Lemma wsubst_cons_equiv (π : {finperm atom}) c a f f' :
     [disjoint finsupp π & Supp] ->
-                  π \dot @wsubst_cons c a f f' = 
+                  π \dot @wsubst_cons c a f f' =
                   @wsubst_cons c a (π \dot f) (π \dot f').
 Proof. by rewrite /wsubst_cons Cons_equivariant. Qed.
 
 Lemma wsubst_bcons_equiv (π : {finperm atom}) c y a f f' :
-    [disjoint finsupp π & Supp] -> 
-    π \dot @wsubst_bcons c y a f f' = 
-    @wsubst_bcons c (π y) a (π \dot f) (π \dot f').    
+    [disjoint finsupp π & Supp] ->
+    π \dot @wsubst_bcons c y a f f' =
+    @wsubst_bcons c (π y) a (π \dot f) (π \dot f').
 Proof. by rewrite /wsubst_bcons BCons_equivariant. Qed.
 
 Lemma FCB y c a f f' : y # Supp -> y # (@wsubst_bcons c y a f f').
@@ -960,8 +961,8 @@ Proof. by rewrite /wsubst W_rect_VarE /wsubst_var. Qed.
 Lemma wsubst_ConsE c a f : wsubst (@Cons c a f) = @Cons c a (wsubst \o f).
 Proof. by rewrite /wsubst W_rect_ConsE /wsubst_cons. Qed.
 
-Lemma wsubst_BConsE c y a f : 
-  y # x -> y # t -> 
+Lemma wsubst_BConsE c y a f :
+  y # x -> y # t ->
   wsubst (@BCons c y a f) = @BCons c y a (wsubst \o f).
 Proof.
 move => yFx yFt.
